src/hott/algebra/bundled.lean
@@ -1,0 +1,126 @@
+/-
+Copyright (c) 2015 Jeremy Avigad. All rights reserved.
+Released under Apache 2.0 license as described in the file LICENSE.
+Authors: Jeremy Avigad
+
+Bundled structures
+-/
+import .ring
+
+universes u v w
+hott_theory
+
+namespace hott
+
+open algebra pointed is_trunc
+
+namespace algebra
+@[hott] structure Semigroup :=
+(carrier : Type _) (struct : semigroup carrier)
+
+@[hott] instance has_coe_to_sort_Semigroup : has_coe_to_sort Semigroup := 
+⟨_, Semigroup.carrier⟩
+attribute [instance] Semigroup.struct 
+
+@[hott] structure CommSemigroup :=
+(carrier : Type _) (struct : comm_semigroup carrier)
+
+@[hott] instance has_coe_to_sort_CommSemigroup : has_coe_to_sort CommSemigroup := 
+⟨_, CommSemigroup.carrier⟩
+attribute [instance] CommSemigroup.struct 
+
+@[hott] structure Monoid :=
+(carrier : Type _) (struct : monoid carrier)
+
+@[hott] instance has_coe_to_sort_Monoid : has_coe_to_sort Monoid := 
+⟨_, Monoid.carrier⟩
+attribute [instance] Monoid.struct 
+
+@[hott] structure CommMonoid :=
+(carrier : Type _) (struct : comm_monoid carrier)
+
+@[hott] instance has_coe_to_sort_CommMonoid : has_coe_to_sort CommMonoid := 
+⟨_, CommMonoid.carrier⟩
+attribute [instance] CommMonoid.struct
+
+@[hott] structure Group :=
+(carrier : Type _) (struct' : group carrier)
+
+attribute [instance] Group.struct' 
+
+@[hott, reducible] def pSet_of_Group (G : Group) : Set* :=
+ptrunctype.mk (pType.mk (Group.carrier G) 1) (semigroup.is_set_carrier _)
+
+@[hott] instance has_coe_Group_pSet : has_coe Group Set* := 
+⟨pSet_of_Group⟩
+
+@[hott, instance, priority 2000] def Group.struct (G : Group) : group G :=
+Group.struct' G
+
+@[hott, reducible] def pType_of_Group (G : Group.{u}) : pType.{u} :=
+↑(↑G : pSet.{u})
+@[hott, reducible] def Set_of_Group (G : Group.{u}) : Set.{u} :=
+↑(↑G : pSet.{u})
+
+@[hott] structure AbGroup :=
+(carrier : Type _) (struct' : ab_group carrier)
+
+attribute [instance] AbGroup.struct'
+
+section
+@[hott] def Group_of_AbGroup (G : AbGroup) : Group :=
+Group.mk G.carrier (ab_group.to_group _)
+
+@[hott] instance has_coe_AbGroup_Group : has_coe AbGroup Group :=
+⟨Group_of_AbGroup⟩
+end
+
+@[hott, instance, priority 2000] def AbGroup.struct (G : AbGroup) : ab_group G :=
+AbGroup.struct' G
+
+-- some bundled infinity-structures
+@[hott] structure InfGroup :=
+(carrier : Type _) (struct' : inf_group carrier)
+
+attribute [instance] InfGroup.struct'
+
+@[hott, reducible] def pType_of_InfGroup (G : InfGroup) : Type* :=
+pType.mk G.carrier 1
+
+@[hott] instance has_coe_InfGroup_pType : has_coe InfGroup Type* :=
+⟨pType_of_InfGroup⟩
+
+@[hott, instance, priority 2000] def InfGroup.struct (G : InfGroup) : inf_group G :=
+InfGroup.struct' G
+
+@[hott] structure AbInfGroup :=
+(carrier : Type _) (struct' : ab_inf_group carrier)
+
+attribute [instance] AbInfGroup.struct'
+
+@[hott] def InfGroup_of_AbInfGroup (G : AbInfGroup) : InfGroup :=
+⟨G.carrier, by apply_instance⟩
+
+@[hott] instance has_coe_AbInfGroup_InfGroup : has_coe AbInfGroup InfGroup :=
+⟨InfGroup_of_AbInfGroup⟩
+
+@[hott, instance, priority 2000] def AbInfGroup.struct (G : AbInfGroup) : ab_inf_group G :=
+G.struct'
+
+@[hott] def InfGroup_of_Group (G : Group) : InfGroup :=
+InfGroup.mk G (by apply_instance)
+
+@[hott] def AbInfGroup_of_AbGroup (G : AbGroup) : AbInfGroup :=
+AbInfGroup.mk G (by apply_instance)
+
+/- rings -/
+@[hott] structure Ring :=
+(carrier : Type _) (struct : ring carrier)
+
+instance has_coe_Ring : has_coe_to_sort Ring.{u} :=
+⟨Type u, Ring.carrier⟩
+attribute [instance] Ring.struct
+
+end algebra
+
+end hott
