src/hott/homotopy/susp.lean
@@ -1,0 +1,520 @@
+/-
+Copyright (c) 2015 Floris van Doorn. All rights reserved.
+Released under Apache 2.0 license as described in the file LICENSE.
+Authors: Floris van Doorn, Ulrik Buchholtz
+
+Declaration of suspension
+-/
+
+import ..hit.pushout ..types.pointed2 ..cubical.square .connectedness
+universes u v w
+
+namespace hott
+hott_theory
+
+open hott.pushout hott.equiv unit pointed hott.is_equiv
+
+@[hott] def susp' (A : Type _) : Type _ := pushout (λ(a : A), star) (λ(a : A), star)
+
+namespace susp
+
+  @[hott] def north' {A : Type _} : susp' A :=
+  inl star
+
+  @[hott, instance] def pointed_susp (X : Type _) : pointed (susp' X) :=
+  pointed.mk north'
+
+end susp open susp
+
+@[hott] def susp (X : Type _) : Type* :=
+pointed.MK (susp' X) north'
+
+@[hott, hsimp] def carrier_susp (X : Type _) : ↥(susp X) = susp' X := by refl
+
+notation `⅀` := susp
+
+namespace susp
+section
+  variable {A : Type _}
+
+  @[hott] def north {A : Type _} : susp A :=
+  north'
+
+  @[hott] def south {A : Type _} : susp A :=
+  inr star
+
+  @[hott] def merid (a : A) : @north A = @south A :=
+  glue a
+
+  @[hott, induction, elab_as_eliminator] protected def rec {P : susp A → Type _} 
+    (PN : P north) (PS : P south) (Pm : Π(a : A), PN =[merid a] PS) (x : susp' A) : P x :=
+  begin
+    hinduction x using pushout.rec with u u,
+    { cases u, exact PN },
+    { cases u, exact PS },
+    { apply Pm },
+  end
+
+  @[hott] theorem rec_merid {P : susp A → Type _} (PN : P north) (PS : P south)
+    (Pm : Π(a : A), PN =[merid a] PS) (a : A)
+      : apd (susp.rec PN PS Pm) (merid a) = Pm a :=
+  begin delta susp.rec, dsimp, exact rec_glue _ _ _ a end
+
+  @[hott, induction] protected def elim {P : Type _} (PN : P) (PS : P) (Pm : A → PN = PS)
+    (x : susp' A) : P :=
+  susp.rec PN PS (λa, pathover_of_eq _ (Pm a)) x
+
+  @[hott] theorem elim_merid {P : Type _} {PN PS : P} (Pm : A → PN = PS) (a : A)
+    : ap (susp.elim PN PS Pm) (merid a) = Pm a :=
+  begin
+    apply eq_of_fn_eq_fn_inv ((pathover_constant (merid a)) _ _),
+    dsimp [susp.elim, susp.rec], refine (apd_eq_pathover_of_eq_ap _ _)⁻¹ ⬝ rec_glue _ _ _ _
+  end
+
+  @[hott] protected def elim_type (PN : Type _) (PS : Type _) (Pm : A → PN ≃ PS)
+    (x : susp' A) : Type _ :=
+  pushout.elim_type (λx, PN) (λx, PS) Pm x
+
+  @[hott] theorem elim_type_merid (PN : Type _) (PS : Type _) (Pm : A → PN ≃ PS)
+    (a : A) : transport (susp.elim_type PN PS Pm) (merid a) = Pm a :=
+  elim_type_glue _ _ _ _
+
+  @[hott] theorem elim_type_merid_inv {A : Type _} (PN : Type _) (PS : Type _) (Pm : A → PN ≃ PS)
+    (a : A) : transport (susp.elim_type PN PS Pm) (merid a)⁻¹ = to_inv (Pm a) :=
+  elim_type_glue_inv _ _ _ _
+
+  @[hott] protected def merid_square {a a' : A} (p : a = a')
+    : square (merid a) (merid a') idp idp :=
+  by induction p; apply vrefl
+
+  open is_trunc is_conn trunc
+  -- theorem 8.2.1
+  @[hott, instance] def is_conn_susp (n : trunc_index) (A : Type _)
+    [H : is_conn n A] : is_conn (n .+1) (susp A) :=
+  is_contr.mk (tr north)
+  begin
+    intro x, hinduction x with x, dsimp at x, hinduction x,
+    { refl },
+    { hinduction center (trunc n A) with p a, exact ap tr (merid a) },
+    { hinduction center (trunc n A) with p a', dsimp,
+      apply pathover_of_tr_eq,
+      rwr [eq_transport_Fr, idp_con],
+      unfreezeI,
+      induction n with n IH generalizing H,
+      { apply is_prop.elim },
+      { change ap (@tr n .+2 (susp A)) (merid a) = ap tr (merid a'),
+        hgeneralize : a' = x,
+        apply is_conn_fun.elim n
+              (is_conn_fun_from_unit n A a)
+              (λx : A, trunctype.mk' n (ap (@tr n .+2 (susp A)) (merid a) = ap tr (merid x))),
+        intros,
+        change ap (@tr n .+2 (susp A)) (merid a) = ap tr (merid a),
+        refl }
+    }
+  end
+end
+  /- Flattening @[hott] lemma -/
+
+  open prod
+  section
+    parameters (A : Type _) (PN PS : Type u) (Pm : A → PN ≃ PS)
+    include Pm
+
+    private abbreviation P := susp.elim_type PN PS Pm
+
+    private abbreviation F : A × PN → PN := λz, z.2
+
+    private abbreviation G : A × PN → PS := λz, Pm z.1 z.2
+
+    @[hott] protected def flattening : sigma P ≃ pushout F G :=
+    begin
+      refine pushout.flattening _ _ _ _ _ ⬝e _,
+      fapply pushout.equiv,
+      { exact sigma.equiv_prod A PN },
+      { apply sigma.sigma_unit_left },
+      { apply sigma.sigma_unit_left },
+      { refl },
+      { refl }
+    end
+  end
+
+end susp
+
+/- Functoriality and equivalence -/
+namespace susp
+  variables {A : Type _} {B : Type _} (f : A → B)
+  include f
+
+  @[hott] def susp_functor' : susp A → susp B :=
+  begin
+    intro x, dsimp at x, hinduction x with a,
+    { exact north },
+    { exact south },
+    { exact merid (f a) }
+  end
+
+  variable [Hf : is_equiv f]
+  include Hf
+
+  open is_equiv
+  @[hott, instance] protected def is_equiv_functor : is_equiv (susp_functor' f) :=
+  adjointify (susp_functor' f) (susp_functor' f⁻¹ᶠ)
+  begin abstract {
+    intro sb, dsimp at sb, hinduction sb with b, refl, refl,
+    apply eq_pathover,
+    rwr [ap_id, ap_compose (susp_functor' f) (susp_functor' f⁻¹ᶠ)],
+    dsimp [susp_functor'], rwr [susp.elim_merid, susp.elim_merid], apply transpose,
+    apply susp.merid_square (right_inv f b)
+   } end
+  begin abstract {
+    intro sa, dsimp at sa, hinduction sa with a, refl, refl,
+    apply eq_pathover,
+    rwr [ap_id, ap_compose (susp_functor' f⁻¹ᶠ) (susp_functor' f)],
+    dsimp [susp_functor'],
+    rwr [susp.elim_merid, susp.elim_merid], apply transpose,
+    apply susp.merid_square (left_inv f a)
+  } end
+
+
+end susp
+
+namespace susp
+  variables {A : Type _} {B : Type _} (f : A ≃ B)
+
+  @[hott] protected def equiv : susp A ≃ susp B :=
+  equiv.mk (susp_functor' f) (susp.is_equiv_functor f)
+end susp
+
+namespace susp
+  open pointed is_trunc
+  variables {X : Type*} {X' : Type*} {Y : Type*} {Y' : Type*} {Z : Type*}
+
+  @[hott] def susp_functor (f : X →* Y) : susp X →* susp Y :=
+  begin
+    fconstructor,
+    { exact susp_functor' f },
+    { refl }
+  end
+
+  @[hott, hsimp] def functor_merid (f : X →* Y) (x : X) : 
+    @ap (susp X) (susp Y) (susp_functor f).to_fun _ _ (merid x) = merid (f.to_fun x) :=
+  elim_merid _ x
+
+  @[hott] def is_equiv_susp_functor (f : X →* Y) [Hf : is_equiv f]
+    : is_equiv (susp_functor f) :=
+  susp.is_equiv_functor f
+
+  @[hott] def susp_pequiv (f : X ≃* Y) : susp X ≃* susp Y :=
+  pequiv_of_equiv (susp.equiv f.to_equiv) idp
+
+set_option pp.coercions true
+  @[hott] def susp_functor_pcompose (g : Y →* Z) (f : X →* Y) :
+    susp_functor (g ∘* f) ~* susp_functor g ∘* susp_functor f :=
+  begin
+    fapply phomotopy.mk,
+    { intro x, dsimp at *, hinduction x,
+      { refl },
+      { refl },
+      { apply eq_pathover, apply hdeg_square,
+        refine functor_merid _ _ ⬝ _ ⬝ (ap_compose (susp_functor g) _ _)⁻¹ᵖ,
+        hsimp, refl }},
+    { refl },
+  end
+
+  @[hott] def susp_functor_phomotopy {f g : X →* Y} (p : f ~* g) :
+    susp_functor f ~* susp_functor g :=
+  begin
+    fapply phomotopy.mk,
+    { intro x, dsimp at *, hinduction x,
+      { refl },
+      { refl },
+      { apply eq_pathover, apply hdeg_square, refine (elim_merid _ _) ⬝ _ ⬝ (elim_merid _ _)⁻¹ᵖ,
+        exact ap merid (p a), }},
+    { refl },
+  end
+
+  @[hott] def susp_functor_pid (A : Type*) : susp_functor (pid A) ~* pid (susp A) :=
+  begin
+    fapply phomotopy.mk,
+    { intro x, dsimp at x, hinduction x,
+      { refl },
+      { refl },
+      { apply eq_pathover_id_right, apply hdeg_square, apply elim_merid }},
+    { refl },
+  end
+
+  /- adjunction originally  ported from Coq-HoTT,
+     but we proved some additional naturality conditions -/
+
+  @[hott] def loop_susp_unit (X : Type*) : X →* Ω(susp X) :=
+  begin
+    fconstructor,
+    { intro x, exact merid x ⬝ (merid pt)⁻¹ },
+    { apply con.right_inv },
+  end
+/-
+ (eq.rec (refl (refl (susp_functor' f ((⅀ X).Point))))
+               (ap (susp_functor' f) ((loop_susp_unit {carrier := X, Point := x}).to_fun x)) ⬝
+             (ap_con (susp_functor' f) (merid x) (merid x)⁻¹ ⬝
+                whisker_left (ap (susp_functor' f) (merid x)) (ap_inv (susp_functor' f) (merid x))) ⬝
+           elim_merid (λ (a : X), merid (f a)) x ◾ (elim_merid (λ (a : X), merid (f a)) x)⁻²)⁻¹ ⬝
+      (ap ((Ω→ (susp_functor {to_fun := f, resp_pt := refl (f x)})).to_fun)
+           ((loop_susp_unit {carrier := X, Point := x}).resp_pt) ⬝
+         (Ω→ (susp_functor {to_fun := f, resp_pt := refl (f x)})).resp_pt) =
+    refl ((loop_susp_unit {carrier := Y, Point := f x}).to_fun (f x)) ⬝
+      (loop_susp_unit {carrier := Y, Point := f x}).resp_pt
+-/
+  @[hott] def loop_susp_unit_natural (f : X →* Y)
+    : loop_susp_unit Y ∘* f ~* Ω→ (susp_functor f) ∘* loop_susp_unit X :=
+  begin
+    induction X with X x, induction Y with Y y, induction f with f pf, dsimp at *, induction pf,
+    fapply phomotopy.mk,
+    { intro x', symmetry,
+      exact
+        ap1_gen_idp_left _ _ ⬝
+        (ap_con _ _ _ ⬝ whisker_left _ (ap_inv _ _)) ⬝
+        elim_merid _ _ ◾ (elim_merid _ _)⁻² },
+    { dsimp [loop_susp_unit, -con.right_inv, -ap1_gen_idp_left], refine _ ⬝ (idp_con _)⁻¹ᵖ,
+      apply inv_con_eq_of_eq_con,
+      refine _ ⬝ con.assoc' _ _ _, rwr inverse2_right_inv,
+      refine _ ⬝ con.assoc' _ _ _,
+      rwr [ap_con_right_inv],
+      rwr [ap1_gen_idp_left_con],
+      rwr [←ap_compose (concat idp)] },
+  end
+
+  @[hott] def loop_susp_counit (X : Type*) : susp (Ω X) →* X :=
+  begin
+    fapply pmap.mk,
+    { intro x, dsimp at x, hinduction x, exact pt, exact pt, exact a },
+    { refl },
+  end
+
+  @[hott] def loop_susp_counit_natural (f : X →* Y)
+    : f ∘* loop_susp_counit X ~* loop_susp_counit Y ∘* (susp_functor (ap1 f)) :=
+  begin
+    induction X with X x, induction Y with Y y, induction f with f pf, dsimp at *, induction pf,
+    fconstructor,
+    { intro x', dsimp at *, hinduction x' with p,
+      { refl },
+      { refl },
+      { apply eq_pathover, apply hdeg_square, dsimp [pcompose, loop_susp_counit],
+        rwr [ap_compose f, ap_compose (susp.elim (f x) (f x) (λ (a : f x = f x), a))],
+        dsimp [susp_functor, susp_functor'], rwr [elim_merid, elim_merid, elim_merid],
+        dsimp [ap1], rwr [ap1_gen_idp_left] }},
+    { refl }
+  end
+
+  @[hott] def loop_susp_counit_unit (X : Type*)
+    : ap1 (loop_susp_counit X) ∘* loop_susp_unit (Ω X) ~* pid (Ω X) :=
+  begin
+    induction X with X x, fconstructor,
+    { intro p, 
+      refine (ap1_gen_idp_left _ _) ⬝
+             (ap_con _ _ _ ⬝
+             whisker_left _ (ap_inv _ _)) ⬝ _,
+      refine (elim_merid _ _ ◾ (elim_merid _ _)⁻²) ⬝ _, refl },
+    { dsimp [loop_susp_unit, -ap1_gen_idp_left, -con.right_inv], 
+      refine idp ◾ ((con_idp _)⁻¹ᵖ ⬝ inverse2_right_inv _) ⬝ _,
+      refine con.assoc _ _ _ ⬝ _,
+      refine whisker_left _ (ap_con_right_inv (susp.elim x x (λa, a)) (merid (refl x))) ⬝ _,
+      rwr [ap1_gen_idp_left_con, ←ap_compose] }
+  end
+
+  @[hott] def loop_susp_unit_counit (X : Type*)
+    : loop_susp_counit (susp X) ∘* susp_functor (loop_susp_unit X) ~* pid (susp X) :=
+  begin
+    induction X with X x, fconstructor,
+    { intro x', dsimp at *, hinduction x',
+      { refl },
+      { exact merid x },
+      { apply eq_pathover, dsimp [pid, pcompose, loop_susp_counit], 
+        refine ap_compose (susp.elim north north (λa, a)) _ _ ⬝ph _ ⬝hp (ap_id _)⁻¹ᵖ,
+        refine ap02 _ (functor_merid _ _) ⬝ elim_merid _ _ ⬝ph _,
+        apply square_of_eq, exact idp_con _ ⬝ (inv_con_cancel_right _ _)⁻¹ }},
+    { refl }
+  end
+
+  @[hott] def susp_elim {X Y : Type*} (f : X →* Ω Y) : susp X →* Y :=
+  loop_susp_counit Y ∘* susp_functor f
+
+  @[hott] def loop_susp_intro {X Y : Type*} (f : susp X →* Y) : X →* Ω Y :=
+  ap1 f ∘* loop_susp_unit X
+
+  @[hott] def susp_elim_susp_functor {A B C : Type*} (g : B →* Ω C) (f : A →* B) :
+    susp_elim g ∘* susp_functor f ~* susp_elim (g ∘* f) :=
+  begin
+    refine passoc _ _ _ ⬝* _, exact pwhisker_left _ (susp_functor_pcompose _ _)⁻¹*
+  end
+
+  @[hott] def susp_elim_phomotopy {A B : Type*} {f g : A →* Ω B} (p : f ~* g) : susp_elim f ~* susp_elim g :=
+  pwhisker_left _ (susp_functor_phomotopy p)
+
+  @[hott] def susp_elim_natural {X Y Z : Type*} (g : Y →* Z) (f : X →* Ω Y)
+    : g ∘* susp_elim f ~* susp_elim (Ω→ g ∘* f) :=
+  begin
+    refine _ ⬝* pwhisker_left _ (susp_functor_pcompose _ _)⁻¹*,
+    refine (passoc _ _ _)⁻¹* ⬝* _ ⬝* passoc _ _ _,
+    exact pwhisker_right _ (loop_susp_counit_natural _)
+  end
+
+  @[hott] def loop_susp_intro_natural {X Y Z : Type*} (g : susp Y →* Z) (f : X →* Y) :
+    loop_susp_intro (g ∘* susp_functor f) ~* loop_susp_intro g ∘* f :=
+  pwhisker_right _ (ap1_pcompose _ _) ⬝* passoc _ _ _ ⬝* 
+  pwhisker_left _ (loop_susp_unit_natural _)⁻¹* ⬝* (passoc _ _ _)⁻¹*
+
+  @[hott] def susp_adjoint_loop_right_inv {X Y : Type*} (g : X →* Ω Y) :
+    loop_susp_intro (susp_elim g) ~* g :=
+  begin
+    refine pwhisker_right _ (ap1_pcompose _ _) ⬝* _,
+    refine passoc _ _ _ ⬝* _,
+    refine pwhisker_left _ (loop_susp_unit_natural _)⁻¹* ⬝* _,
+    refine (passoc _ _ _)⁻¹* ⬝* _,
+    refine pwhisker_right _ (loop_susp_counit_unit _) ⬝* _,
+    apply pid_pcompose
+  end
+
+  @[hott] def susp_adjoint_loop_left_inv {X Y : Type*} (f : susp X →* Y) :
+    susp_elim (loop_susp_intro f) ~* f :=
+  begin
+    refine pwhisker_left _ (susp_functor_pcompose _ _) ⬝* _,
+    refine (passoc _ _ _)⁻¹* ⬝* _,
+    refine pwhisker_right _ (loop_susp_counit_natural _)⁻¹* ⬝* _,
+    refine passoc _ _ _ ⬝* _,
+    refine pwhisker_left _ (loop_susp_unit_counit _) ⬝* _,
+    apply pcompose_pid
+  end
+
+  @[hott] def susp_adjoint_loop_unpointed (X Y : Type*) : susp X →* Y ≃ X →* Ω Y :=
+  begin
+    fapply equiv.MK,
+    { exact loop_susp_intro },
+    { exact susp_elim },
+    { intro g, apply eq_of_phomotopy, exact susp_adjoint_loop_right_inv g },
+    { intro f, apply eq_of_phomotopy, exact susp_adjoint_loop_left_inv f }
+  end
+
+  @[hott] def susp_functor_pconst_homotopy {X Y : Type*} (x : susp X) :
+    susp_functor (pconst X Y) x = pt :=
+  begin
+    dsimp at x, hinduction x,
+    { refl },
+    { exact (merid pt)⁻¹ },
+    { apply eq_pathover, refine (elim_merid _ _) ⬝ph _ ⬝hp (ap_constant _ _)⁻¹, exact square_of_eq (con.right_inv _)⁻¹ }
+  end
+
+  @[hott] def susp_functor_pconst (X Y : Type*) : susp_functor (pconst X Y) ~* pconst (susp X) (susp Y) :=
+  begin
+    fapply phomotopy.mk,
+    { exact susp_functor_pconst_homotopy },
+    { refl }
+  end
+
+  @[hott] def susp_pfunctor (X Y : Type*) : ppmap X Y →* ppmap (susp X) (susp Y) :=
+  pmap.mk susp_functor (eq_of_phomotopy (susp_functor_pconst _ _))
+
+  @[hott] def susp_pelim (X Y : Type*) : ppmap X (Ω Y) →* ppmap (susp X) Y :=
+  ppcompose_left (loop_susp_counit Y) ∘* susp_pfunctor X (Ω Y)
+
+  @[hott] def loop_susp_pintro (X Y : Type*) : ppmap (susp X) Y →* ppmap X (Ω Y) :=
+  ppcompose_right (loop_susp_unit X) ∘* pap1 (susp X) Y
+
+  @[hott] def loop_susp_pintro_natural_left (f : X' →* X) :
+    psquare (loop_susp_pintro X Y) (loop_susp_pintro X' Y)
+            (ppcompose_right (susp_functor f)) (ppcompose_right f) :=
+  pap1_natural_left _ ⬝h* ppcompose_right_psquare (loop_susp_unit_natural f)⁻¹*
+
+  @[hott] def loop_susp_pintro_natural_right (f : Y →* Y') :
+    psquare (loop_susp_pintro X Y) (loop_susp_pintro X Y')
+            (ppcompose_left f) (ppcompose_left (Ω→ f)) :=
+  pap1_natural_right _ ⬝h* (ppcompose_left_ppcompose_right _ _)⁻¹*
+
+  @[hott] def is_equiv_loop_susp_pintro (X Y : Type*) :
+    is_equiv (loop_susp_pintro X Y) :=
+  begin
+    fapply adjointify,
+    { exact susp_pelim X Y },
+    { intro g, apply eq_of_phomotopy, exact susp_adjoint_loop_right_inv g },
+    { intro f, apply eq_of_phomotopy, exact susp_adjoint_loop_left_inv f }
+  end
+
+  -- @[hott] def susp_adjoint_loop (X Y : Type*) : ppmap (susp X) Y ≃* ppmap X (Ω Y) :=
+  -- pequiv_of_pmap (loop_susp_pintro X Y) (is_equiv_loop_susp_pintro X Y)
+
+  -- @[hott] def susp_adjoint_loop_natural_right (f : Y →* Y') :
+  --   psquare (susp_adjoint_loop X Y).to_pmap (susp_adjoint_loop X Y').to_pmap
+  --           (ppcompose_left f) (ppcompose_left (Ω→ f)) :=
+  -- loop_susp_pintro_natural_right f
+
+  -- @[hott] def susp_adjoint_loop_natural_left (f : X' →* X) :
+  --   psquare (susp_adjoint_loop X Y).to_pmap (susp_adjoint_loop X' Y).to_pmap
+  --           (ppcompose_right (susp_functor f)) (ppcompose_right f) :=
+  -- loop_susp_pintro_natural_left f
+
+  -- @[hott] def ap1_susp_elim {A : Type*} {X : Type*} (p : A →* Ω X) :
+  --   Ω→(susp_elim p) ∘* loop_susp_unit A ~* p :=
+  -- susp_adjoint_loop_right_inv p
+
+  -- /- the underlying homotopies of susp_adjoint_loop_natural_* -/
+  -- @[hott] def susp_adjoint_loop_nat_right (f : susp X →* Y) (g : Y →* Z)
+  --   : (susp_adjoint_loop X Z).to_pmap (g ∘* f) ~* ap1 g ∘* (susp_adjoint_loop X Y).to_pmap f :=
+  -- begin
+  --   dsimp [susp_adjoint_loop],
+  --   refine _ ⬝* passoc _ _ _,
+  --   apply pwhisker_right,
+  --   apply ap1_pcompose
+  -- end
+
+  -- @[hott] def susp_adjoint_loop_nat_left (f : Y →* Ω Z) (g : X →* Y)
+  --   : (susp_adjoint_loop X Z)⁻¹ᵉ (f ∘* g) ~* (susp_adjoint_loop Y Z)⁻¹ᵉ f ∘* susp_functor g :=
+  -- begin
+  --   esimp [susp_adjoint_loop],
+  --   refine _ ⬝* (passoc _ _ _)⁻¹*,
+  --   apply pwhisker_left,
+  --   apply susp_functor_pcompose
+  -- end
+
+  -- /- iterated suspension -/
+  -- @[hott] def iterate_susp (n : ℕ) (A : Type*) : Type* := iterate (λX, susp X) n A
+
+  -- open is_conn trunc_index nat
+  -- @[hott] def iterate_susp_succ (n : ℕ) (A : Type*) :
+  --   iterate_susp (succ n) A = susp (iterate_susp n A) :=
+  -- idp
+
+  -- @[hott] def is_conn_iterate_susp [instance] (n : ℕ₋₂) (m : ℕ) (A : Type*)
+  --   [H : is_conn n A] : is_conn (n + m) (iterate_susp m A) :=
+  -- begin induction m with m IH, exact H, exact @is_conn_susp _ _ IH end
+
+  -- -- Separate cases for n = 0, which comes up often
+  -- @[hott] def is_conn_iterate_susp_zero [instance] (m : ℕ) (A : Type*)
+  --   [H : is_conn 0 A] : is_conn m (iterate_susp m A) :=
+  -- begin induction m with m IH, exact H, exact @is_conn_susp _ _ IH end
+
+  -- @[hott] def iterate_susp_functor (n : ℕ) {A B : Type*} (f : A →* B) :
+  --   iterate_susp n A →* iterate_susp n B :=
+  -- begin
+  --   induction n with n g,
+  --   { exact f },
+  --   { exact susp_functor g }
+  -- end
+
+  -- @[hott] def iterate_susp_succ_in (n : ℕ) (A : Type*) :
+  --   iterate_susp (succ n) A ≃* iterate_susp n (susp A) :=
+  -- begin
+  --   induction n with n IH,
+  --   { refl},
+  --   { exact susp_pequiv IH}
+  -- end
+
+  -- @[hott] def iterate_susp_adjoint_loopn (X Y : Type*) (n : ℕ) :
+  --   ppmap (iterate_susp n X) Y ≃* ppmap X (Ω[n] Y) :=
+  -- begin
+  --   induction n with n IH generalizing X Y,
+  --   { refl },
+  --   { refine susp_adjoint_loop _ _ ⬝e* IH _ _ ⬝e* _, apply pequiv_ppcompose_left,
+  --     symmetry, apply loopn_succ_in }
+  -- end
+
+end susp
+end hott
