changes.md
@@ -17,4 +17,4 @@ There are many differences between Lean 2 and Lean 3 which will break Lean 2 fil
 * `eq_of_homotopy_eta` removed (was duplicate of `eq_of_homotopy_apd10`)
 * remove `*_on` eliminators for HITs.
 * `ptrunctype`, `pconntype`, `ptruncconntype` have a pointed type as field (not a type and a point as two separate fields)
-<!-- (to do) * renamed `eq_of_fn_eq_fn` to `inj` -->
+<!-- (to do) * renamed `eq_of_fn_eq_fn` to `inj` and `pathover_of_pathover_ap` to `pathover_compose` -->
