src/hott/algebra/e_closure.hlean
@@ -1,0 +1,243 @@
+/-
+Copyright (c) 2015 Floris van Doorn. All rights reserved.
+Released under Apache 2.0 license as described in the file LICENSE.
+Author: Floris van Doorn
+
+The "equivalence closure" of a type-valued relation.
+A more appropriate intuition is the type of words formed from the relation,
+  and inverses, concatenations and reflexivity
+-/
+
+import algebra.relation eq2 arity cubical.pathover2
+
+open eq equiv function
+
+inductive e_closure {A : Type _} (R : A → A → Type _) : A → A → Type _ :=
+| of_rel : Π{a a'} (r : R a a'), e_closure R a a'
+| of_path : Π{a a'} (pp : a = a'), e_closure R a a'
+| symm : Π{a a'} (r : e_closure R a a'), e_closure R a' a
+| trans : Π{a a' a''} (r : e_closure R a a') (r' : e_closure R a' a''), e_closure R a a''
+
+namespace e_closure
+  infix ` ⬝r `:75 := e_closure.trans
+  postfix `⁻¹ʳ`:(max+10) := e_closure.symm
+  notation `[`:max a `]`:0 := e_closure.of_rel a
+  notation `<`:max p `>`:0 := e_closure.of_path _ p
+  abbreviation rfl {A : Type _} {R : A → A → Type _} {a : A} := of_path R (idpath a)
+end e_closure
+open e_closure
+namespace relation
+
+section
+  parameters {A : Type _}
+             {R : A → A → Type _}
+  local abbreviation T := e_closure R
+
+  variables ⦃a a' a'' : A⦄ {s : R a a'} {r : T a a} {B C : Type _}
+
+  @[hott] protected def e_closure.elim {f : A → B}
+    (e : Π⦃a a' : A⦄, R a a' → f a = f a') (t : T a a') : f a = f a' :=
+  begin
+    induction t with a a' r a a' pp a a' r IH a a' a'' r r' IH₁ IH₂,
+      exact e r,
+      exact ap f pp,
+      exact IH⁻¹,
+      exact IH₁ ⬝ IH₂
+  end
+
+  @[hott] def ap_e_closure_elim_h {B C : Type _} {f : A → B} {g : B → C}
+    (e : Π⦃a a' : A⦄, R a a' → f a = f a')
+    {e' : Π⦃a a' : A⦄, R a a' → g (f a) = g (f a')}
+    (p : Π⦃a a' : A⦄ (s : R a a'), ap g (e s) = e' s) (t : T a a')
+    : ap g (e_closure.elim e t) = e_closure.elim e' t :=
+  begin
+    induction t with a a' r a a' pp a a' r IH a a' a'' r r' IH₁ IH₂,
+      apply p,
+      induction pp, reflexivity,
+      exact ap_inv g (e_closure.elim e r) ⬝ inverse2 IH,
+      exact ap_con g (e_closure.elim e r) (e_closure.elim e r') ⬝ (IH₁ ◾ IH₂)
+  end
+
+  @[hott] def ap_e_closure_elim_h_symm {B C : Type _} {f : A → B} {g : B → C}
+    {e : Π⦃a a' : A⦄, R a a' → f a = f a'}
+    {e' : Π⦃a a' : A⦄, R a a' → g (f a) = g (f a')}
+    (p : Π⦃a a' : A⦄ (s : R a a'), ap g (e s) = e' s) (t : T a a') :
+    ap_e_closure_elim_h e p t⁻¹ʳ = ap_inv g (e_closure.elim e t) ⬝ (ap_e_closure_elim_h e p t)⁻² :=
+  by reflexivity
+
+  @[hott] def ap_e_closure_elim_h_trans {B C : Type _} {f : A → B} {g : B → C}
+    {e : Π⦃a a' : A⦄, R a a' → f a = f a'}
+    {e' : Π⦃a a' : A⦄, R a a' → g (f a) = g (f a')}
+    (p : Π⦃a a' : A⦄ (s : R a a'), ap g (e s) = e' s) (t : T a a') (t' : T a' a'')
+    : ap_e_closure_elim_h e p (t ⬝r t') = ap_con g (e_closure.elim e t) (e_closure.elim e t') ⬝
+      (ap_e_closure_elim_h e p t ◾ ap_e_closure_elim_h e p t') :=
+  by reflexivity
+
+  @[hott] def ap_e_closure_elim {B C : Type _} {f : A → B} (g : B → C)
+    (e : Π⦃a a' : A⦄, R a a' → f a = f a') (t : T a a')
+    : ap g (e_closure.elim e t) = e_closure.elim (λa a' r, ap g (e r)) t :=
+  ap_e_closure_elim_h e (λa a' s, idp) t
+
+  @[hott] def ap_e_closure_elim_symm {B C : Type _} {f : A → B} (g : B → C)
+    (e : Π⦃a a' : A⦄, R a a' → f a = f a') (t : T a a')
+    : ap_e_closure_elim g e t⁻¹ʳ = ap_inv g (e_closure.elim e t) ⬝ (ap_e_closure_elim g e t)⁻² :=
+  by reflexivity
+
+  @[hott] def ap_e_closure_elim_trans {B C : Type _} {f : A → B} (g : B → C)
+    (e : Π⦃a a' : A⦄, R a a' → f a = f a') (t : T a a') (t' : T a' a'')
+    : ap_e_closure_elim g e (t ⬝r t') = ap_con g (e_closure.elim e t) (e_closure.elim e t') ⬝
+      (ap_e_closure_elim g e t ◾ ap_e_closure_elim g e t') :=
+  by reflexivity
+
+  @[hott] def e_closure_elim_eq {f : A → B}
+    {e e' : Π⦃a a' : A⦄, R a a' → f a = f a'} (p : e ~3 e') (t : T a a')
+    : e_closure.elim e t = e_closure.elim e' t :=
+  begin
+    induction t with a a' r a a' pp a a' r IH a a' a'' r r' IH₁ IH₂,
+      apply p,
+      reflexivity,
+      exact IH⁻²,
+      exact IH₁ ◾ IH₂
+  end
+
+  -- TODO: formulate and prove this without using function extensionality,
+  -- and modify the proofs using this to also not use function extensionality
+  -- strategy: use `e_closure_elim_eq` instead of `ap ... (eq_of_homotopy3 p)`
+  @[hott] def ap_e_closure_elim_h_eq {B C : Type _} {f : A → B} {g : B → C}
+    (e : Π⦃a a' : A⦄, R a a' → f a = f a')
+    {e' : Π⦃a a' : A⦄, R a a' → g (f a) = g (f a')}
+    (p : Π⦃a a' : A⦄ (s : R a a'), ap g (e s) = e' s) (t : T a a')
+    : ap_e_closure_elim_h e p t =
+      ap_e_closure_elim g e t ⬝ ap (λx, e_closure.elim x t) (eq_of_homotopy3 p) :=
+  begin
+    fapply homotopy3.rec_on p,
+    intro q, esimp at q, induction q,
+    esimp, rewrite eq_of_homotopy3_id
+  end
+
+  @[hott] theorem ap_ap_e_closure_elim_h {B C D : Type _} {f : A → B}
+    {g : B → C} (h : C → D)
+    (e : Π⦃a a' : A⦄, R a a' → f a = f a')
+    {e' : Π⦃a a' : A⦄, R a a' → g (f a) = g (f a')}
+    (p : Π⦃a a' : A⦄ (s : R a a'), ap g (e s) = e' s) (t : T a a')
+    : square (ap (ap h) (ap_e_closure_elim_h e p t))
+             (ap_e_closure_elim_h e (λa a' s, ap_compose h g (e s)) t)
+             (ap_compose h g (e_closure.elim e t))⁻¹
+             (ap_e_closure_elim_h e' (λa a' s, (ap (ap h) (p s))⁻¹) t) :=
+  begin
+    induction t with a a' r a a' pp a a' r IH a a' a'' r r' IH₁ IH₂,
+    { esimp,
+      apply square_of_eq, exact !con.right_inv ⬝ !con.left_inv⁻¹},
+    { induction pp, apply ids},
+    { rewrite [▸*,ap_con (ap h)],
+      refine (transpose !ap_compose_inv)⁻¹ᵛ ⬝h _,
+      rewrite [con_inv,inv_inv,-inv2_inv],
+      exact !ap_inv2 ⬝v square_inv2 IH},
+    { rewrite [▸*,ap_con (ap h)],
+      refine (transpose !ap_compose_con)⁻¹ᵛ ⬝h _,
+      rewrite [con_inv,inv_inv,con2_inv],
+      refine !ap_con2 ⬝v square_con2 IH₁ IH₂},
+  end
+
+  @[hott] theorem ap_ap_e_closure_elim {B C D : Type _} {f : A → B}
+    (g : B → C) (h : C → D)
+    (e : Π⦃a a' : A⦄, R a a' → f a = f a') (t : T a a')
+    : square (ap (ap h) (ap_e_closure_elim g e t))
+             (ap_e_closure_elim_h e (λa a' s, ap_compose h g (e s)) t)
+             (ap_compose h g (e_closure.elim e t))⁻¹
+             (ap_e_closure_elim   h (λa a' r, ap g (e r)) t) :=
+  !ap_ap_e_closure_elim_h
+
+  @[hott] def ap_e_closure_elim_h_zigzag {B C D : Type _} {f : A → B}
+    {g : B → C} (h : C → D)
+    (e : Π⦃a a' : A⦄, R a a' → f a = f a')
+    {e' : Π⦃a a' : A⦄, R a a' → h (g (f a)) = h (g (f a'))}
+    (p : Π⦃a a' : A⦄ (s : R a a'), ap (h ∘ g) (e s) = e' s) (t : T a a')
+    : ap_e_closure_elim   h (λa a' s, ap g (e s)) t ⬝
+     (ap_e_closure_elim_h e (λa a' s, ap_compose h g (e s)) t)⁻¹ ⬝
+      ap_e_closure_elim_h e p t =
+      ap_e_closure_elim_h (λa a' s, ap g (e s)) (λa a' s, (ap_compose h g (e s))⁻¹ ⬝ p s) t :=
+  begin
+    refine whisker_right _ (eq_of_square (ap_ap_e_closure_elim g h e t)⁻¹ʰ)⁻¹ ⬝ _,
+    refine !con.assoc ⬝ _, apply inv_con_eq_of_eq_con, apply eq_of_square,
+    apply transpose,
+    -- the rest of the proof is almost the same as the proof of ap_ap_e_closure_elim[_h].
+    -- Is there a connection between these theorems?
+    induction t with a a' r a a' pp a a' r IH a a' a'' r r' IH₁ IH₂,
+    { esimp, apply square_of_eq, apply idp_con},
+    { induction pp, apply ids},
+    { rewrite [▸*,ap_con (ap h)],
+      refine (transpose !ap_compose_inv)⁻¹ᵛ ⬝h _,
+      rewrite [con_inv,inv_inv,-inv2_inv],
+      exact !ap_inv2 ⬝v square_inv2 IH},
+    { rewrite [▸*,ap_con (ap h)],
+      refine (transpose !ap_compose_con)⁻¹ᵛ ⬝h _,
+      rewrite [con_inv,inv_inv,con2_inv],
+      refine !ap_con2 ⬝v square_con2 IH₁ IH₂},
+
+  end
+
+  @[hott] def is_equivalence_e_closure : is_equivalence T :=
+  begin
+    constructor,
+      intro a, exact rfl,
+      intros a a' t, exact t⁻¹ʳ,
+      intros a a' a'' t t', exact t ⬝r t',
+  end
+
+  /- dependent elimination -/
+
+  variables {P : B → Type _} {Q : C → Type _} {f : A → B} {g : B → C} {f' : Π(a : A), P (f a)}
+  @[hott] protected def e_closure.elimo (p : Π⦃a a' : A⦄, R a a' → f a = f a')
+    (po : Π⦃a a' : A⦄ (s : R a a'), f' a =[p s] f' a') (t : T a a')
+    : f' a =[e_closure.elim p t] f' a' :=
+  begin
+    induction t with a a' r a a' pp a a' r IH a a' a'' r r' IH₁ IH₂,
+      exact po r,
+      induction pp, constructor,
+      exact IH⁻¹ᵒ,
+      exact IH₁ ⬝o IH₂
+  end
+
+  @[hott] def elimo_symm (p : Π⦃a a' : A⦄, R a a' → f a = f a')
+    (po : Π⦃a a' : A⦄ (s : R a a'), f' a =[p s] f' a') (t : T a a')
+    : e_closure.elimo p po t⁻¹ʳ = (e_closure.elimo p po t)⁻¹ᵒ :=
+  by reflexivity
+
+  @[hott] def elimo_trans (p : Π⦃a a' : A⦄, R a a' → f a = f a')
+    (po : Π⦃a a' : A⦄ (s : R a a'), f' a =[p s] f' a') (t : T a a') (t' : T a' a'')
+    : e_closure.elimo p po (t ⬝r t') = e_closure.elimo p po t ⬝o e_closure.elimo p po t' :=
+  by reflexivity
+
+  @[hott] def ap_e_closure_elimo_h  {g' : Πb, Q (g b)}
+    (p : Π⦃a a' : A⦄, R a a' → f a = f a')
+    (po : Π⦃a a' : A⦄ (s : R a a'), g' (f a) =[p s] g' (f a'))
+    (q : Π⦃a a' : A⦄ (s : R a a'), apd g' (p s) = po s)
+    (t : T a a') : apd g' (e_closure.elim p t) = e_closure.elimo p po t :=
+  begin
+    induction t with a a' r a a' pp a a' r IH a a' a'' r r' IH₁ IH₂,
+      apply q,
+      induction pp, reflexivity,
+      esimp [e_closure.elim],
+      exact apd_inv g' (e_closure.elim p r) ⬝ IH⁻²ᵒ,
+      exact apd_con g' (e_closure.elim p r) (e_closure.elim p r') ⬝ (IH₁ ◾o IH₂)
+  end
+
+  @[hott] theorem e_closure_elimo_ap {g' : Π(a : A), Q (g (f a))}
+    (p : Π⦃a a' : A⦄, R a a' → f a = f a')
+    (po : Π⦃a a' : A⦄ (s : R a a'), g' a =[ap g (p s)] g' a')
+    (t : T a a') : e_closure.elimo p (λa a' s, pathover_of_pathover_ap Q g (po s)) t =
+      pathover_of_pathover_ap Q g (change_path (ap_e_closure_elim g p t)⁻¹
+        (e_closure.elimo (λa a' r, ap g (p r)) po t)) :=
+  begin
+    induction t with a a' r a a' pp a a' r IH a a' a'' r r' IH₁ IH₂,
+    { reflexivity},
+    { induction pp; reflexivity},
+    { rewrite [+elimo_symm, ap_e_closure_elim_symm, IH, con_inv, change_path_con, ▸*, -inv2_inv,
+               change_path_invo, pathover_of_pathover_ap_invo]},
+    { rewrite [+elimo_trans, ap_e_closure_elim_trans, IH₁, IH₂, con_inv, change_path_con, ▸*,
+               con2_inv, change_path_cono, pathover_of_pathover_ap_cono]},
+  end
+
+end
+end relation
