src/hott/algebra/group_power.hlean
@@ -1,0 +1,357 @@
+/-
+Copyright (c) 2015 Jeremy Avigad. All rights reserved.
+Released under Apache 2.0 license as described in the file LICENSE.
+Author: Jeremy Avigad
+
+The power operation on monoids prod groups. We separate this from group, because it depends on
+nat, which in turn depends on other parts of algebra.
+
+We have "pow a n" for natural number powers, prod "gpow a i" for integer powers. The notation
+a^n is used for the first, but users can locally redefine it to gpow when needed.
+
+Note: power adopts the convention that 0^0=1.
+-/
+import types.nat.basic types.int.basic .homomorphism .group_theory
+open algebra
+
+namespace algebra
+variables {A B : Type _}
+
+structure has_pow_nat [class] (A : Type _) :=
+(pow_nat : A → nat → A)
+
+@[hott] def pow_nat {A : Type _} [s : has_pow_nat A] : A → nat → A :=
+has_pow_nat.pow_nat
+
+infix ` ^ ` := pow_nat
+
+structure has_pow_int [class] (A : Type _) :=
+(pow_int : A → int → A)
+
+@[hott] def pow_int {A : Type _} [s : has_pow_int A] : A → int → A :=
+has_pow_int.pow_int
+
+ /- monoid -/
+section monoid
+open nat
+
+variable [s : monoid A]
+include s
+
+@[hott] def monoid.pow (a : A) : ℕ → A
+| 0     := 1
+| (n+1) := a * monoid.pow n
+
+@[hott] def monoid_has_pow_nat [instance] : has_pow_nat A :=
+has_pow_nat.mk monoid.pow
+
+@[hott] theorem pow_zero (a : A) : a^0 = 1 := rfl
+@[hott] theorem pow_succ (a : A) (n : ℕ) : a^(succ n) = a * a^n := rfl
+
+@[hott] theorem pow_one (a : A) : a^1 = a := !mul_one
+@[hott] theorem pow_two (a : A) : a^2 = a * a :=
+calc
+  a^2 = a * (a * 1) : rfl
+  ... = a * a       : mul_one
+@[hott] theorem pow_three (a : A) : a^3 = a * (a * a) :=
+calc
+  a^3 = a * (a * (a * 1)) : rfl
+  ... = a * (a * a)       : mul_one
+@[hott] theorem pow_four (a : A) : a^4 = a * (a * (a * a))  :=
+calc
+  a^4 = a * a^3           : rfl
+  ... = a * (a * (a * a)) : pow_three
+
+@[hott] theorem pow_succ' (a : A) : Πn, a^(succ n) = a^n * a
+| 0        := by rewrite [pow_succ, *pow_zero, one_mul, mul_one]
+| (succ n) := by rewrite [pow_succ, pow_succ' at {1}, pow_succ, mul.assoc]
+
+@[hott] theorem one_pow : Π n : ℕ, 1^n = (1:A)
+| 0        := rfl
+| (succ n) := by rewrite [pow_succ, one_mul, one_pow]
+
+@[hott] theorem pow_add (a : A) (m n : ℕ) : a^(m + n) = a^m * a^n :=
+begin
+  induction n with n ih,
+    {krewrite [nat.add_zero, pow_zero, mul_one]},
+  rewrite [add_succ, *pow_succ', ih, mul.assoc]
+end
+
+@[hott] theorem pow_mul (a : A) (m : ℕ) : Π n, a^(m * n) = (a^m)^n
+| 0        := by rewrite [nat.mul_zero, pow_zero]
+| (succ n) := by rewrite [nat.mul_succ, pow_add, pow_succ', pow_mul]
+
+@[hott] theorem pow_comm (a : A) (m n : ℕ)  : a^m * a^n = a^n * a^m :=
+by rewrite [-*pow_add, add.comm]
+
+end monoid
+
+/- commutative monoid -/
+
+section comm_monoid
+open nat
+variable [s : comm_monoid A]
+include s
+
+@[hott] theorem mul_pow (a b : A) : Π n, (a * b)^n = a^n * b^n
+| 0        := by rewrite [*pow_zero, mul_one]
+| (succ n) := by rewrite [*pow_succ', mul_pow, *mul.assoc, mul.left_comm a]
+
+end comm_monoid
+
+section group
+variable [s : group A]
+include s
+
+section nat
+open nat
+@[hott] theorem inv_pow (a : A) : Πn, (a⁻¹)^n = (a^n)⁻¹
+| 0        := by rewrite [*pow_zero, one_inv]
+| (succ n) := by rewrite [pow_succ, pow_succ', inv_pow, mul_inv]
+@[hott] theorem pow_sub (a : A) {m n : ℕ} (H : m ≥ n) : a^(m - n) = a^m * (a^n)⁻¹ :=
+have H1 : m - n + n = m, from nat.sub_add_cancel H,
+have H2 : a^(m - n) * a^n = a^m, by rewrite [-pow_add, H1],
+eq_mul_inv_of_mul_eq H2
+
+@[hott] theorem pow_inv_comm (a : A) : Πm n, (a⁻¹)^m * a^n = a^n * (a⁻¹)^m
+| 0 n               := by rewrite [*pow_zero, one_mul, mul_one]
+| m 0               := by rewrite [*pow_zero, one_mul, mul_one]
+| (succ m) (succ n) := by rewrite [pow_succ' at {1}, pow_succ at {1}, pow_succ', pow_succ,
+                            *mul.assoc, inv_mul_cancel_left, mul_inv_cancel_left, pow_inv_comm]
+
+@[hott] lemma respect_pow [group B] (f : A → B) [is_mul_hom f] (a : A) : Πn, f (a ^ n) = (f a) ^ n
+| 0        := respect_one f
+| (succ n) := by rewrite [pow_succ, respect_mul, respect_pow]
+
+end nat
+
+open int
+
+@[hott] def gpow (a : A) : ℤ → A
+| (of_nat n) := a^n
+| -[1+n]     := (a^(nat.succ n))⁻¹
+
+open nat
+
+@[hott] lemma gpow_zero (a : A) : gpow a 0 = 1 := rfl
+@[hott] lemma gpow_one (a : A) : gpow a 1 = a := pow_one a
+@[hott] lemma gpow_eq_pow (a : A) (n : ℕ) : gpow a n = a^n := by reflexivity
+
+private @[hott] lemma gpow_add_aux (a : A) (m n : ℕ) :
+  gpow a ((of_nat m) + -[1+n]) = gpow a (of_nat m) * gpow a (-[1+n]) :=
+sum.elim (nat.lt_sum_ge m (nat.succ n))
+  (assume H : (m < nat.succ n),
+    have H1 : (#nat nat.succ n - m > nat.zero), from nat.sub_pos_of_lt H,
+    calc
+      gpow a ((of_nat m) + -[1+n]) = gpow a (sub_nat_nat m (nat.succ n))  : rfl
+        ... = gpow a (-[1+ nat.pred (nat.sub (nat.succ n) m)])            : {sub_nat_nat_of_lt H}
+        ... = (a ^ (nat.succ (nat.pred (nat.sub (nat.succ n) m))))⁻¹    : rfl
+        ... = (a ^ (nat.succ n) * (a ^ m)⁻¹)⁻¹                        :
+                by krewrite [succ_pred_of_pos H1, pow_sub a (nat.le_of_lt H)]
+        ... = a ^ m * (a ^ (nat.succ n))⁻¹                            :
+                by rewrite [mul_inv, inv_inv]
+        ... = gpow a (of_nat m) * gpow a (-[1+n])                         : rfl)
+  (assume H : (m ≥ nat.succ n),
+    calc
+      gpow a ((of_nat m) + -[1+n]) = gpow a (sub_nat_nat m (nat.succ n))  : rfl
+        ... = gpow a (#nat m - nat.succ n)                                : {sub_nat_nat_of_ge H}
+        ... = a ^ m * (a ^ (nat.succ n))⁻¹                                : pow_sub a H
+        ... = gpow a (of_nat m) * gpow a (-[1+n])                         : rfl)
+
+@[hott] theorem gpow_add (a : A) : Πi j : int, gpow a (i + j) = gpow a i * gpow a j
+| (of_nat m) (of_nat n) := !pow_add
+| (of_nat m) -[1+n]     := !gpow_add_aux
+| -[1+m]     (of_nat n) := by rewrite [add.comm, gpow_add_aux, ↑gpow, -*inv_pow, pow_inv_comm]
+| -[1+m]     -[1+n]     :=
+  calc
+    gpow a (-[1+m] + -[1+n]) = (a^(#nat nat.succ m + nat.succ n))⁻¹ : rfl
+      ... = (a^(nat.succ m))⁻¹ * (a^(nat.succ n))⁻¹ : by rewrite [pow_add, pow_comm, mul_inv]
+      ... = gpow a (-[1+m]) * gpow a (-[1+n])       : rfl
+
+@[hott] theorem gpow_comm (a : A) (i j : ℤ) : gpow a i * gpow a j = gpow a j * gpow a i :=
+by rewrite [-*gpow_add, add.comm]
+
+@[hott] lemma gpow_neg (a : A) : Π(n : ℤ), gpow a (-n) = (gpow a n)⁻¹
+| (of_nat n) := by cases n with n; rewrite [gpow_zero,one_inv]; reflexivity
+| -[1+n]     := by rewrite [↑gpow at {2}, inv_inv]
+
+@[hott] lemma inv_gpow (a : A) : Π(n : ℤ), gpow a⁻¹ n = (gpow a n)⁻¹
+| (of_nat n) := !inv_pow
+| -[1+n]     := by rewrite [↑gpow, inv_pow]
+
+private @[hott] lemma gpow_mul_aux (a : A) (m n : ℕ) :
+  gpow a ((of_nat m) * -[1+n]) = gpow (gpow a (of_nat m)) (-[1+n]) :=
+by rewrite [↑gpow at {2,3}, -pow_mul, -gpow_eq_pow, -gpow_neg]
+
+@[hott] theorem gpow_mul (a : A) : Π n m, gpow a (n * m) = gpow (gpow a n) m
+| (of_nat m) (of_nat n) := !pow_mul
+| (of_nat m) -[1+n]     := by rewrite [↑gpow at {2,3}, -pow_mul, -gpow_eq_pow, -gpow_neg]
+| -[1+m]     (of_nat n) := by rewrite [↑gpow at {2,3}, inv_pow, -pow_mul, -gpow_eq_pow, -gpow_neg]
+| -[1+m]     -[1+n]     := by rewrite [↑gpow at {2,3}, inv_pow, inv_inv, -pow_mul]
+
+@[hott] lemma respect_gpow [group B] (f : A → B) [is_mul_hom f] (a : A) : Πn, f (gpow a n) = gpow (f a) n
+| (of_nat n) := !respect_pow
+| -[1+n]     := by rewrite [↑gpow, respect_inv, respect_pow]
+
+end group
+
+section comm_monoid
+open int
+variable [ab_group A]
+
+@[hott] theorem mul_gpow (a b : A) : Πi, gpow (a * b) i = gpow a i * gpow b i
+| (of_nat n) := !mul_pow
+| -[1+n]     := by rewrite [↑gpow,-mul_inv,mul.comm,mul_pow]
+
+end comm_monoid
+
+section ordered_ring
+open nat
+variable [s : linear_ordered_ring A]
+include s
+
+@[hott] theorem pow_pos {a : A} (H : a > 0) (n : ℕ) : a ^ n > 0 :=
+  begin
+    induction n,
+    krewrite pow_zero,
+    apply zero_lt_one,
+    rewrite pow_succ',
+    apply mul_pos,
+    apply v_0, apply H
+  end
+
+@[hott] theorem pow_ge_one_of_ge_one {a : A} (H : a ≥ 1) (n : ℕ) : a ^ n ≥ 1 :=
+  begin
+    induction n,
+    krewrite pow_zero,
+    apply le.refl,
+    rewrite [pow_succ', -mul_one 1],
+    apply mul_le_mul v_0 H zero_le_one,
+    apply le_of_lt,
+    apply pow_pos,
+    apply gt_of_ge_of_gt H zero_lt_one
+  end
+
+@[hott] theorem pow_two_add (n : ℕ) : (2:A)^n + 2^n = 2^(succ n) :=
+  by rewrite [pow_succ', -one_add_one_eq_two, left_distrib, *mul_one]
+
+end ordered_ring
+
+section bundled
+open group
+@[hott] lemma to_respect_pow {A B : Group} (f : A →g B) (a : A) (n : ℕ) : f (a ^ n) = (f a) ^ n :=
+respect_pow f a n
+
+@[hott] lemma to_respect_gpow {A B : Group} (f : A →g B) (a : A) (n : ℤ) : f (gpow a n) = gpow (f a) n :=
+respect_gpow f a n
+end bundled
+
+/- additive monoid -/
+
+section add_monoid
+variable [s : add_monoid A]
+include s
+local attribute add_monoid.to_monoid [trans_instance]
+open nat
+
+@[hott] def nmul : ℕ → A → A := λ n a, a^n
+
+local infix [priority algebra.prio] `⬝` := nmul
+
+@[hott] theorem zero_nmul (a : A) : (0:ℕ) ⬝ a = 0 := pow_zero a
+@[hott] theorem succ_nmul (n : ℕ) (a : A) : nmul (succ n) a = a + (nmul n a) := pow_succ a n
+
+@[hott] theorem succ_nmul' (n : ℕ) (a : A) : succ n ⬝ a = nmul n a + a := pow_succ' a n
+
+@[hott] theorem nmul_zero (n : ℕ) : n ⬝ 0 = (0:A) := one_pow n
+
+@[hott] theorem one_nmul (a : A) : 1 ⬝ a = a := pow_one a
+
+@[hott] theorem add_nmul (m n : ℕ) (a : A) : (m + n) ⬝ a = (m ⬝ a) + (n ⬝ a) := pow_add a m n
+
+@[hott] theorem mul_nmul (m n : ℕ) (a : A) : (m * n) ⬝ a = m ⬝ (n ⬝ a) :=
+eq.subst (mul.comm n m) (pow_mul a n m)
+
+@[hott] theorem nmul_comm (m n : ℕ) (a : A) : (m ⬝ a) + (n ⬝ a) = (n ⬝ a) + (m ⬝ a) := pow_comm a m n
+
+end add_monoid
+
+namespace ops
+infix [priority algebra.prio] `⬝` := nmul
+end ops
+open algebra.ops
+/- additive commutative monoid -/
+
+section add_comm_monoid
+open nat
+variable [s : add_comm_monoid A]
+include s
+local attribute add_comm_monoid.to_comm_monoid [trans_instance]
+
+@[hott] theorem nmul_add (n : ℕ) (a b : A) : n ⬝ (a + b) = (n ⬝ a) + (n ⬝ b) := mul_pow a b n
+
+end add_comm_monoid
+
+section add_group
+variable [s : add_group A]
+include s
+local attribute add_group.to_group [trans_instance]
+
+section nat
+open nat
+@[hott] theorem nmul_neg (n : ℕ) (a : A) : n ⬝ (-a) = -(n ⬝ a) := inv_pow a n
+
+@[hott] theorem sub_nmul {m n : ℕ} (a : A) (H : m ≥ n) : (m - n) ⬝ a = (m ⬝ a) + -(n ⬝ a) := pow_sub a H
+
+@[hott] theorem nmul_neg_comm (m n : ℕ) (a : A) : (m ⬝ (-a)) + (n ⬝ a) = (n ⬝ a) + (m ⬝ (-a)) :=
+pow_inv_comm a m n
+
+@[hott] lemma respect_nmul [add_group B] (f : A → B) [H : is_add_hom f] (n : ℕ) (a : A) :
+  f (nmul n a) = nmul n (f a) :=
+to_respect_pow (group.homomorphism.mk f H) a n
+
+end nat
+
+open int
+
+@[hott] def imul : ℤ → A → A := λ i a, gpow a i
+
+@[hott] theorem add_imul (i j : ℤ) (a : A) : imul (i + j) a = imul i a + imul j a :=
+  gpow_add a i j
+
+@[hott] theorem imul_comm (i j : ℤ) (a : A) : imul i a + imul j a = imul j a + imul i a := gpow_comm a i j
+
+end add_group
+
+section add_ab_group
+open int
+variable [add_ab_group A]
+local attribute add_ab_group.to_ab_group [trans_instance]
+
+@[hott] theorem imul_add (i : ℤ) (a b : A) : imul i (a + b) = imul i a + imul i b :=
+mul_gpow a b i
+
+@[hott] theorem mul_imul (i j : ℤ) (a : A) : imul (i * j) a = imul i (imul j a) :=
+by rewrite [mul.comm]; apply gpow_mul
+
+@[hott] lemma one_imul (a : A) : imul 1 a = a :=
+gpow_one a
+
+@[hott] lemma respect_imul [add_group B] (f : A → B) [H : is_add_hom f] (n : ℤ) (a : A) :
+  f (imul n a) = imul n (f a) :=
+to_respect_gpow (group.homomorphism.mk f H) a n
+
+end add_ab_group
+
+section bundled
+open group
+
+@[hott] lemma to_respect_nmul {A B : AddGroup} (f : A →g B) (n : ℕ) (a : A) : f (nmul n a) = nmul n (f a) :=
+to_respect_pow f a n
+
+@[hott] lemma to_respect_imul {A B : AddGroup} (f : A →g B) (n : ℤ) (a : A) : f (imul n a) = imul n (f a) :=
+to_respect_gpow f a n
+
+end bundled
+
+end algebra
