src/hott/algebra/group_theory.hlean
@@ -1,0 +1,594 @@
+/-
+Copyright (c) 2015 Floris van Doorn. All rights reserved.
+Released under Apache 2.0 license as described in the file LICENSE.
+Authors: Floris van Doorn
+
+Basic group theory
+-/
+
+import algebra.category.category algebra.bundled .homomorphism
+
+open eq algebra pointed function is_trunc pi equiv is_equiv
+set_option class.force_new true
+
+namespace group
+  @[hott] def pointed_Group [instance] (G : Group) : pointed G :=
+  pointed.mk 1
+
+  @[hott] def Group.struct' [instance] [reducible] (G : Group) : group G :=
+  Group.struct G
+
+  @[hott] def ab_group_pSet_of_Group [instance] (G : AbGroup) : ab_group (pSet_of_Group G) :=
+  AbGroup.struct G
+
+  @[hott] def group_pSet_of_Group [instance] [priority 900] (G : Group) :
+    group (pSet_of_Group G) :=
+  Group.struct G
+
+  /- left and right actions -/
+  @[hott] def is_equiv_mul_right {A : Group} (a : A) : is_equiv (λb, b * a) :=
+  adjointify _ (λb : A, b * a⁻¹) (λb, !inv_mul_cancel_right) (λb, !mul_inv_cancel_right)
+
+  @[hott] def right_action {A : Group} (a : A) : A ≃ A :=
+  equiv.mk _ (is_equiv_mul_right a)
+
+  @[hott] def is_equiv_add_right {A : AddGroup} (a : A) : is_equiv (λb, b + a) :=
+  adjointify _ (λb : A, b - a) (λb, !neg_add_cancel_right) (λb, !add_neg_cancel_right)
+
+  @[hott] def add_right_action {A : AddGroup} (a : A) : A ≃ A :=
+  equiv.mk _ (is_equiv_add_right a)
+
+  /- homomorphisms -/
+
+  structure homomorphism (G₁ G₂ : Group) : Type _ :=
+    (φ : G₁ → G₂)
+    (p : is_mul_hom φ)
+
+  infix ` →g `:55 := homomorphism
+
+  abbreviation group_fun [coercion] [reducible] := @homomorphism.φ
+  @[hott] def homomorphism.struct [instance] [priority 900] {G₁ G₂ : Group}
+    (φ : G₁ →g G₂) : is_mul_hom φ :=
+  homomorphism.p φ
+
+  @[hott] def homomorphism.mulstruct [instance] [priority 2000] {G₁ G₂ : Group} (φ : G₁ →g G₂)
+    : is_mul_hom φ :=
+  homomorphism.p φ
+
+  @[hott] def homomorphism.addstruct [instance] [priority 2000] {G₁ G₂ : AddGroup} (φ : G₁ →g G₂)
+    : is_add_hom φ :=
+  homomorphism.p φ
+
+  variables {G G₁ G₂ G₃ : Group} {g h : G₁} {ψ : G₂ →g G₃} {φ₁ φ₂ : G₁ →g G₂} (φ : G₁ →g G₂)
+
+  @[hott] def to_respect_mul /- φ -/ (g h : G₁) : φ (g * h) = φ g * φ h :=
+  respect_mul φ g h
+
+  @[hott] theorem to_respect_one /- φ -/ : φ 1 = 1 :=
+  respect_one φ
+
+  @[hott] theorem to_respect_inv /- φ -/ (g : G₁) : φ g⁻¹ = (φ g)⁻¹ :=
+  respect_inv φ g
+
+  @[hott] def to_is_embedding_homomorphism /- φ -/ (H : Π{g}, φ g = 1 → g = 1) : is_embedding φ :=
+  is_embedding_of_is_mul_hom φ @H
+
+  variables (G₁ G₂)
+  @[hott] def is_set_homomorphism [instance] : is_set (G₁ →g G₂) :=
+  begin
+    have H : G₁ →g G₂ ≃ Σ(f : G₁ → G₂), Π(g₁ g₂ : G₁), f (g₁ * g₂) = f g₁ * f g₂,
+    begin
+      fapply equiv.MK,
+      { intro φ, induction φ, constructor, exact (respect_mul φ)},
+      { intro v, induction v with f H, constructor, exact H},
+      { intro v, induction v, reflexivity},
+      { intro φ, induction φ, reflexivity}
+    end,
+    apply is_trunc_equiv_closed_rev, exact H
+  end
+
+  variables {G₁ G₂}
+  @[hott] def pmap_of_homomorphism /- φ -/ : G₁ →* G₂ :=
+  pmap.mk φ begin esimp, exact respect_one φ end
+
+  @[hott] def homomorphism_change_fun {G₁ G₂ : Group}
+    (φ : G₁ →g G₂) (f : G₁ → G₂) (p : φ ~ f) : G₁ →g G₂ :=
+  homomorphism.mk f
+    (λg h, (p (g * h))⁻¹ ⬝ to_respect_mul φ g h ⬝ ap011 mul (p g) (p h))
+
+  @[hott] def homomorphism_eq (p : φ₁ ~ φ₂) : φ₁ = φ₂ :=
+  begin
+    induction φ₁ with φ₁ q₁, induction φ₂ with φ₂ q₂, esimp at p, induction p,
+    exact ap (homomorphism.mk φ₁) !is_prop.elim
+  end
+
+  section additive
+  variables {H₁ H₂ : AddGroup} (χ : H₁ →g H₂)
+  @[hott] def to_respect_add /- χ -/ (g h : H₁) : χ (g + h) = χ g + χ h :=
+  respect_add χ g h
+
+  @[hott] theorem to_respect_zero /- χ -/ : χ 0 = 0 :=
+  respect_zero χ
+
+  @[hott] theorem to_respect_neg /- χ -/ (g : H₁) : χ (-g) = -(χ g) :=
+  respect_neg χ g
+
+  end additive
+
+  section add_mul
+  variables {H₁ : AddGroup} {H₂ : Group} (χ : H₁ →g H₂)
+  @[hott] def to_respect_add_mul /- χ -/ (g h : H₁) : χ (g + h) = χ g * χ h :=
+  to_respect_mul χ g h
+
+  @[hott] theorem to_respect_zero_one /- χ -/ : χ 0 = 1 :=
+  to_respect_one χ
+
+  @[hott] theorem to_respect_neg_inv /- χ -/ (g : H₁) : χ (-g) = (χ g)⁻¹ :=
+  to_respect_inv χ g
+
+  end add_mul
+
+  section mul_add
+  variables  {H₁ : Group} {H₂ : AddGroup} (χ : H₁ →g H₂)
+  @[hott] def to_respect_mul_add /- χ -/ (g h : H₁) : χ (g * h) = χ g + χ h :=
+  to_respect_mul χ g h
+
+  @[hott] theorem to_respect_one_zero /- χ -/ : χ 1 = 0 :=
+  to_respect_one χ
+
+  @[hott] theorem to_respect_inv_neg /- χ -/ (g : H₁) : χ g⁻¹ = -(χ g) :=
+  to_respect_inv χ g
+
+  end mul_add
+
+  /- categorical structure of groups + homomorphisms -/
+
+  @[hott] def homomorphism_compose [trans] [reducible] (ψ : G₂ →g G₃) (φ : G₁ →g G₂) : G₁ →g G₃ :=
+  homomorphism.mk (ψ ∘ φ) (is_mul_hom_compose _ _)
+
+  variable (G)
+  @[hott] def homomorphism_id [refl] : G →g G :=
+  homomorphism.mk (@id G) (is_mul_hom_id G)
+  variable {G}
+
+  abbreviation gid := @homomorphism_id
+  infixr ` ∘g `:75 := homomorphism_compose
+  notation 1       := homomorphism_id _
+
+  structure isomorphism (A B : Group) :=
+    (to_hom : A →g B)
+    (is_equiv_to_hom : is_equiv to_hom)
+
+  infix ` ≃g `:25 := isomorphism
+  attribute isomorphism.to_hom [coercion]
+  attribute isomorphism.is_equiv_to_hom [instance]
+  attribute isomorphism._trans_of_to_hom
+
+  @[hott] def equiv_of_isomorphism (φ : G₁ ≃g G₂) : G₁ ≃ G₂ :=
+  equiv.mk φ _
+
+  @[hott] def pequiv_of_isomorphism (φ : G₁ ≃g G₂) :
+    G₁ ≃* G₂ :=
+  pequiv.mk φ begin esimp, exact _ end begin esimp, exact respect_one φ end
+
+  @[hott] def isomorphism_of_equiv (φ : G₁ ≃ G₂)
+    (p : Πg₁ g₂, φ (g₁ * g₂) = φ g₁ * φ g₂) : G₁ ≃g G₂ :=
+  isomorphism.mk (homomorphism.mk φ p) !to_is_equiv
+
+  @[hott] def isomorphism_of_eq {G₁ G₂ : Group} (φ : G₁ = G₂) : G₁ ≃g G₂ :=
+  isomorphism_of_equiv (equiv_of_eq (ap Group.carrier φ))
+    begin intros, induction φ, reflexivity end
+
+  @[hott] def to_ginv (φ : G₁ ≃g G₂) : G₂ →g G₁ :=
+  homomorphism.mk φ⁻¹
+    abstract begin
+    intros g₁ g₂, apply eq_of_fn_eq_fn' φ,
+    rewrite [respect_mul φ, +right_inv φ]
+    end end
+
+  variable (G)
+  @[hott] def isomorphism.refl [refl] : G ≃g G :=
+  isomorphism.mk 1 !is_equiv_id
+  variable {G}
+
+  @[hott] def isomorphism.symm [symm] (φ : G₁ ≃g G₂) : G₂ ≃g G₁ :=
+  isomorphism.mk (to_ginv φ) !is_equiv_inv
+
+  @[hott] def isomorphism.trans [trans] (φ : G₁ ≃g G₂) (ψ : G₂ ≃g G₃) : G₁ ≃g G₃ :=
+  isomorphism.mk (ψ ∘g φ) !is_equiv_compose
+
+  @[hott] def isomorphism.eq_trans [trans]
+     {G₁ G₂ : Group} {G₃ : Group} (φ : G₁ = G₂) (ψ : G₂ ≃g G₃) : G₁ ≃g G₃ :=
+  proof isomorphism.trans (isomorphism_of_eq φ) ψ qed
+
+  @[hott] def isomorphism.trans_eq [trans]
+    {G₁ : Group} {G₂ G₃ : Group} (φ : G₁ ≃g G₂) (ψ : G₂ = G₃) : G₁ ≃g G₃ :=
+  isomorphism.trans φ (isomorphism_of_eq ψ)
+
+  postfix `⁻¹ᵍ`:(max + 1) := isomorphism.symm
+  infixl ` ⬝g `:75 := isomorphism.trans
+  infixl ` ⬝gp `:75 := isomorphism.trans_eq
+  infixl ` ⬝pg `:75 := isomorphism.eq_trans
+
+  @[hott] def pmap_of_isomorphism (φ : G₁ ≃g G₂) : G₁ →* G₂ :=
+  pequiv_of_isomorphism φ
+
+  @[hott] def to_fun_isomorphism_trans {G H K : Group} (φ : G ≃g H) (ψ : H ≃g K) :
+    φ ⬝g ψ ~ ψ ∘ φ :=
+  by reflexivity
+
+  @[hott] def add_homomorphism (G H : AddGroup) : Type _ := homomorphism G H
+  infix ` →a `:55 := add_homomorphism
+
+  abbreviation agroup_fun [coercion] [reducible] {G H : AddGroup} (φ : G →a H) : G → H :=
+  φ
+
+  @[hott] def add_homomorphism.struct [instance] {G H : AddGroup} (φ : G →a H) : is_add_hom φ :=
+  homomorphism.addstruct φ
+
+  @[hott] def add_homomorphism.mk {G H : AddGroup} (φ : G → H) (h : is_add_hom φ) : G →g H :=
+  homomorphism.mk φ h
+
+  @[hott] def add_homomorphism_compose [trans] [reducible] {G₁ G₂ G₃ : AddGroup}
+    (ψ : G₂ →a G₃) (φ : G₁ →a G₂) : G₁ →a G₃ :=
+  add_homomorphism.mk (ψ ∘ φ) (is_add_hom_compose _ _)
+
+  @[hott] def add_homomorphism_id [refl] (G : AddGroup) : G →a G :=
+  add_homomorphism.mk (@id G) (is_add_hom_id G)
+
+  abbreviation aid := @add_homomorphism_id
+  infixr ` ∘a `:75 := add_homomorphism_compose
+
+  @[hott] def to_respect_add' {H₁ H₂ : AddGroup} (χ : H₁ →a H₂) (g h : H₁) : χ (g + h) = χ g + χ h :=
+  respect_add χ g h
+
+  @[hott] theorem to_respect_zero' {H₁ H₂ : AddGroup} (χ : H₁ →a H₂) : χ 0 = 0 :=
+  respect_zero χ
+
+  @[hott] theorem to_respect_neg' {H₁ H₂ : AddGroup} (χ : H₁ →a H₂) (g : H₁) : χ (-g) = -(χ g) :=
+  respect_neg χ g
+
+  @[hott] def homomorphism_add {G H : AddAbGroup} (φ ψ : G →a H) : G →a H :=
+  add_homomorphism.mk (λg, φ g + ψ g)
+    abstract begin
+      intros g g', refine ap011 add !to_respect_add' !to_respect_add' ⬝ _,
+      refine !add.assoc ⬝ ap (add _) (!add.assoc⁻¹ ⬝ ap (λx, x + _) !add.comm ⬝ !add.assoc) ⬝ !add.assoc⁻¹
+    end end
+
+  @[hott] def homomorphism_mul {G H : AbGroup} (φ ψ : G →g H) : G →g H :=
+  homomorphism.mk (λg, φ g * ψ g) (to_respect_add (homomorphism_add φ ψ))
+
+  @[hott] def pmap_of_homomorphism_gid (G : Group) : pmap_of_homomorphism (gid G) ~* pid G :=
+  begin
+    fapply phomotopy_of_homotopy, reflexivity
+  end
+
+  @[hott] def pmap_of_homomorphism_gcompose {G H K : Group} (ψ : H →g K) (φ : G →g H)
+    : pmap_of_homomorphism (ψ ∘g φ) ~* pmap_of_homomorphism ψ ∘* pmap_of_homomorphism φ :=
+  begin
+    fapply phomotopy_of_homotopy, reflexivity
+  end
+
+  @[hott] def pmap_of_homomorphism_phomotopy {G H : Group} {φ ψ : G →g H} (H : φ ~ ψ)
+    : pmap_of_homomorphism φ ~* pmap_of_homomorphism ψ :=
+  begin
+    fapply phomotopy_of_homotopy, exact H
+  end
+
+  @[hott] def pequiv_of_isomorphism_trans {G₁ G₂ G₃ : Group} (φ : G₁ ≃g G₂) (ψ : G₂ ≃g G₂) :
+    pequiv_of_isomorphism (φ ⬝g ψ) ~* pequiv_of_isomorphism ψ ∘* pequiv_of_isomorphism φ :=
+  begin
+    apply phomotopy_of_homotopy, reflexivity
+  end
+
+  @[hott] def isomorphism_eq {G H : Group} {φ ψ : G ≃g H} (p : φ ~ ψ) : φ = ψ :=
+  begin
+    induction φ with φ φe, induction ψ with ψ ψe,
+    exact apd011 isomorphism.mk (homomorphism_eq p) !is_prop.elimo
+  end
+
+  @[hott] def is_set_isomorphism [instance] (G H : Group) : is_set (G ≃g H) :=
+  begin
+    have H : G ≃g H ≃ Σ(f : G →g H), is_equiv f,
+    begin
+      fapply equiv.MK,
+      { intro φ, induction φ, constructor, assumption },
+      { intro v, induction v, constructor, assumption },
+      { intro v, induction v, reflexivity },
+      { intro φ, induction φ, reflexivity }
+    end,
+    apply is_trunc_equiv_closed_rev, exact H
+  end
+
+  @[hott] def trivial_homomorphism (A B : Group) : A →g B :=
+  homomorphism.mk (λa, 1) (λa a', (mul_one 1)⁻¹)
+
+  @[hott] def trivial_add_homomorphism (A B : AddGroup) : A →a B :=
+  homomorphism.mk (λa, 0) (λa a', (add_zero 0)⁻¹)
+
+
+  /- given an equivalence A ≃ B we can transport a group structure on A to a group structure on B -/
+
+  section
+
+    parameters {A B : Type _} (f : A ≃ B) [group A]
+
+    @[hott] def group_equiv_mul (b b' : B) : B := f (f⁻¹ᶠ b * f⁻¹ᶠ b')
+
+    @[hott] def group_equiv_one : B := f one
+
+    @[hott] def group_equiv_inv (b : B) : B := f (f⁻¹ᶠ b)⁻¹
+
+    local infix * := group_equiv_mul
+    local postfix ^ := group_equiv_inv
+    local notation 1 := group_equiv_one
+
+    @[hott] theorem group_equiv_mul_assoc (b₁ b₂ b₃ : B) : (b₁ * b₂) * b₃ = b₁ * (b₂ * b₃) :=
+    by rewrite [↑group_equiv_mul, +left_inv f, mul.assoc]
+
+    @[hott] theorem group_equiv_one_mul (b : B) : 1 * b = b :=
+    by rewrite [↑group_equiv_mul, ↑group_equiv_one, left_inv f, one_mul, right_inv f]
+
+    @[hott] theorem group_equiv_mul_one (b : B) : b * 1 = b :=
+    by rewrite [↑group_equiv_mul, ↑group_equiv_one, left_inv f, mul_one, right_inv f]
+
+    @[hott] theorem group_equiv_mul_left_inv (b : B) : b^ * b = 1 :=
+    by rewrite [↑group_equiv_mul, ↑group_equiv_one, ↑group_equiv_inv,
+                +left_inv f, mul.left_inv]
+
+    @[hott] def group_equiv_closed : group B :=
+    ⦃group,
+      mul          := group_equiv_mul,
+      mul_assoc    := group_equiv_mul_assoc,
+      one          := group_equiv_one,
+      one_mul      := group_equiv_one_mul,
+      mul_one      := group_equiv_mul_one,
+      inv          := group_equiv_inv,
+      mul_left_inv := group_equiv_mul_left_inv,
+    is_set_carrier := is_trunc_equiv_closed 0 f⦄
+
+  end
+
+  section
+    variables {A B : Type _} (f : A ≃ B) [ab_group A]
+    @[hott] def group_equiv_mul_comm (b b' : B) : group_equiv_mul f b b' = group_equiv_mul f b' b :=
+    by rewrite [↑group_equiv_mul, mul.comm]
+
+    @[hott] def ab_group_equiv_closed : ab_group B :=
+    ⦃ab_group, group_equiv_closed f,
+      mul_comm := group_equiv_mul_comm f⦄
+  end
+
+  variable (G)
+
+  /- the trivial group -/
+  open unit
+  @[hott] def group_unit : group unit :=
+  group.mk _ (λx y, star) (λx y z, idp) star (unit.rec idp) (unit.rec idp) (λx, star) (λx, idp)
+
+  @[hott] def ab_group_unit : ab_group unit :=
+  ⦃ab_group, group_unit, mul_comm := λx y, idp⦄
+
+  @[hott] def trivial_group : Group :=
+  Group.mk _ group_unit
+
+  abbreviation G0 := trivial_group
+
+  @[hott] def AbGroup_of_Group.{u} (G : Group.{u}) (H : Π x y : G, x * y = y * x) : AbGroup.{u} :=
+  begin
+    induction G,
+    fapply AbGroup.mk,
+    assumption,
+    exact ⦃ab_group, struct', mul_comm := H⦄
+  end
+
+  @[hott] def trivial_ab_group : AbGroup.{0} :=
+  begin
+    fapply AbGroup_of_Group trivial_group, intros x y, reflexivity
+  end
+
+  @[hott] def trivial_group_of_is_contr [H : is_contr G] : G ≃g G0 :=
+  begin
+    fapply isomorphism_of_equiv,
+    { apply equiv_unit_of_is_contr},
+    { intros, reflexivity}
+  end
+
+  @[hott] def ab_group_of_is_contr (A : Type _) [is_contr A] : ab_group A :=
+  have ab_group unit, from ab_group_unit,
+  ab_group_equiv_closed (equiv_unit_of_is_contr A)⁻¹ᵉ
+
+  @[hott] def group_of_is_contr (A : Type _) [is_contr A] : group A :=
+  have ab_group A, from ab_group_of_is_contr A, by apply _
+
+  @[hott] def ab_group_lift_unit : ab_group (lift unit) :=
+  ab_group_of_is_contr (lift unit)
+
+  @[hott] def trivial_ab_group_lift : AbGroup :=
+  AbGroup.mk _ ab_group_lift_unit
+
+  @[hott] def from_trivial_ab_group (A : AbGroup) : trivial_ab_group →g A :=
+  trivial_homomorphism trivial_ab_group A
+
+  @[hott] def is_embedding_from_trivial_ab_group (A : AbGroup) :
+    is_embedding (from_trivial_ab_group A) :=
+  begin
+    fapply is_embedding_of_is_injective,
+    intros x y p,
+    induction x, induction y, reflexivity
+  end
+
+  @[hott] def to_trivial_ab_group (A : AbGroup) : A →g trivial_ab_group :=
+  trivial_homomorphism A trivial_ab_group
+
+  variable {G}
+
+  /-
+    A group where the point in the pointed type corresponds with 1 in the group.
+    We need this structure when we are given a pointed type, and want to say that there is a group
+    structure on it which is compatible with the point. This is used in chain complexes.
+  -/
+  structure pgroup [class] (X : Type*) extends semigroup X, has_inv X :=
+    (pt_mul : Πa, mul pt a = a)
+    (mul_pt : Πa, mul a pt = a)
+    (mul_left_inv_pt : Πa, mul (inv a) a = pt)
+
+  @[hott] def group_of_pgroup [reducible] [instance] (X : Type*) [H : pgroup X]
+    : group X :=
+  ⦃group, H,
+          one := pt,
+          one_mul := pgroup.pt_mul ,
+          mul_one := pgroup.mul_pt,
+          mul_left_inv := pgroup.mul_left_inv_pt⦄
+
+  @[hott] def pgroup_of_group (X : Type*) [H : group X] (p : one = pt :> X) : pgroup X :=
+  begin
+    cases X with X x, esimp at *, induction p,
+    exact ⦃pgroup, H,
+            pt_mul := one_mul,
+            mul_pt := mul_one,
+            mul_left_inv_pt := mul.left_inv⦄
+  end
+
+  @[hott] def Group_of_pgroup (G : Type*) [pgroup G] : Group :=
+  Group.mk G _
+
+  @[hott] def pgroup_Group [instance] (G : Group) : pgroup G :=
+  ⦃ pgroup, Group.struct G,
+    pt_mul := one_mul,
+    mul_pt := mul_one,
+    mul_left_inv_pt := mul.left_inv ⦄
+
+  -- infinity pgroups
+
+  structure inf_pgroup [class] (X : Type*) extends inf_semigroup X, has_inv X :=
+    (pt_mul : Πa, mul pt a = a)
+    (mul_pt : Πa, mul a pt = a)
+    (mul_left_inv_pt : Πa, mul (inv a) a = pt)
+
+  @[hott] def inf_group_of_inf_pgroup [reducible] [instance] (X : Type*) [H : inf_pgroup X]
+    : inf_group X :=
+  ⦃inf_group, H,
+          one := pt,
+          one_mul := inf_pgroup.pt_mul ,
+          mul_one := inf_pgroup.mul_pt,
+          mul_left_inv := inf_pgroup.mul_left_inv_pt⦄
+
+  @[hott] def inf_pgroup_of_inf_group (X : Type*) [H : inf_group X] (p : one = pt :> X) : inf_pgroup X :=
+  begin
+    cases X with X x, esimp at *, induction p,
+    exact ⦃inf_pgroup, H,
+            pt_mul := one_mul,
+            mul_pt := mul_one,
+            mul_left_inv_pt := mul.left_inv⦄
+  end
+
+  @[hott] def inf_Group_of_inf_pgroup (G : Type*) [inf_pgroup G] : InfGroup :=
+  InfGroup.mk G _
+
+  @[hott] def inf_pgroup_InfGroup [instance] (G : InfGroup) : inf_pgroup G :=
+  ⦃ inf_pgroup, InfGroup.struct G,
+    pt_mul := one_mul,
+    mul_pt := mul_one,
+    mul_left_inv_pt := mul.left_inv ⦄
+
+  /- equality of groups and abelian groups -/
+
+  @[hott] def group.to_has_mul {A : Type _} (H : group A) : has_mul A := _
+  @[hott] def group.to_has_inv {A : Type _} (H : group A) : has_inv A := _
+  @[hott] def group.to_has_one {A : Type _} (H : group A) : has_one A := _
+  local attribute group.to_has_mul group.to_has_inv [coercion]
+
+  universe variable l
+  variables {A B : Type l}
+  @[hott] def group_eq {G H : group A} (same_mul' : Π(g h : A), @mul A G g h = @mul A H g h)
+    : G = H :=
+  begin
+    have foo : Π(g : A), @inv A G g = (@inv A G g * g) * @inv A H g,
+      from λg, !mul_inv_cancel_right⁻¹,
+    cases G with Gs Gm Gh1 G1 Gh2 Gh3 Gi Gh4,
+    cases H with Hs Hm Hh1 H1 Hh2 Hh3 Hi Hh4,
+    have same_mul : Gm = Hm, from eq_of_homotopy2 same_mul',
+    cases same_mul,
+    have same_one : G1 = H1, from calc
+      G1 = Hm G1 H1 : Hh3
+     ... = H1 : Gh2,
+    have same_inv : Gi = Hi, from eq_of_homotopy (take g, calc
+      Gi g = Hm (Hm (Gi g) g) (Hi g) : foo
+       ... = Hm G1 (Hi g) : by rewrite Gh4
+       ... = Hi g : Gh2),
+    cases same_one, cases same_inv,
+    have ps  : Gs  = Hs,  from !is_prop.elim,
+    have ph1 : Gh1 = Hh1, from !is_prop.elim,
+    have ph2 : Gh2 = Hh2, from !is_prop.elim,
+    have ph3 : Gh3 = Hh3, from !is_prop.elim,
+    have ph4 : Gh4 = Hh4, from !is_prop.elim,
+    cases ps, cases ph1, cases ph2, cases ph3, cases ph4, reflexivity
+  end
+
+  @[hott] def group_pathover {G : group A} {H : group B} {p : A = B}
+    (resp_mul : Π(g h : A), cast p (g * h) = cast p g * cast p h) : G =[p] H :=
+  begin
+    induction p,
+    apply pathover_idp_of_eq, exact group_eq (resp_mul)
+  end
+
+  @[hott] def Group_eq_of_eq {G H : Group} (p : Group.carrier G = Group.carrier H)
+    (resp_mul : Π(g h : G), cast p (g * h) = cast p g * cast p h) : G = H :=
+  begin
+    cases G with Gc G, cases H with Hc H,
+    apply (apd011 Group.mk p),
+    exact group_pathover resp_mul
+  end
+
+  @[hott] def Group_eq {G H : Group} (f : Group.carrier G ≃ Group.carrier H)
+    (resp_mul : Π(g h : G), f (g * h) = f g * f h) : G = H :=
+  Group_eq_of_eq (ua f) (λg h, !cast_ua ⬝ resp_mul g h ⬝ ap011 mul !cast_ua⁻¹ !cast_ua⁻¹)
+
+  @[hott] def eq_of_isomorphism {G₁ G₂ : Group} (φ : G₁ ≃g G₂) : G₁ = G₂ :=
+  Group_eq (equiv_of_isomorphism φ) (respect_mul φ)
+
+  @[hott] def ab_group.to_has_mul {A : Type _} (H : ab_group A) : has_mul A := _
+  local attribute ab_group.to_has_mul [coercion]
+
+  @[hott] def ab_group_eq {A : Type _} {G H : ab_group A}
+    (same_mul : Π(g h : A), @mul A G g h = @mul A H g h)
+    : G = H :=
+  begin
+    have g_eq : @ab_group.to_group A G = @ab_group.to_group A H, from group_eq same_mul,
+    cases G with Gs Gm Gh1 G1 Gh2 Gh3 Gi Gh4 Gh5,
+    cases H with Hs Hm Hh1 H1 Hh2 Hh3 Hi Hh4 Hh5,
+    have pm : Gm = Hm, from ap (@mul _ ∘ group.to_has_mul) g_eq,
+    have pi : Gi = Hi, from ap (@inv _ ∘ group.to_has_inv) g_eq,
+    have p1 : G1 = H1, from ap (@one _ ∘ group.to_has_one) g_eq,
+    induction pm, induction pi, induction p1,
+    have ps  : Gs  = Hs,  from !is_prop.elim,
+    have ph1 : Gh1 = Hh1, from !is_prop.elim,
+    have ph2 : Gh2 = Hh2, from !is_prop.elim,
+    have ph3 : Gh3 = Hh3, from !is_prop.elim,
+    have ph4 : Gh4 = Hh4, from !is_prop.elim,
+    have ph5 : Gh5 = Hh5, from !is_prop.elim,
+    induction ps, induction ph1, induction ph2, induction ph3, induction ph4, induction ph5,
+    reflexivity
+  end
+
+  @[hott] def ab_group_pathover {A B : Type _} {G : ab_group A} {H : ab_group B} {p : A = B}
+    (resp_mul : Π(g h : A), cast p (g * h) = cast p g * cast p h) : G =[p] H :=
+  begin
+    induction p,
+    apply pathover_idp_of_eq, exact ab_group_eq (resp_mul)
+  end
+
+  @[hott] def AbGroup_eq_of_isomorphism {G₁ G₂ : AbGroup} (φ : G₁ ≃g G₂) : G₁ = G₂ :=
+  begin
+    induction G₁, induction G₂,
+    apply apd011 AbGroup.mk (ua (equiv_of_isomorphism φ)),
+    apply ab_group_pathover,
+    intros g h, exact !cast_ua ⬝ respect_mul φ g h ⬝ ap011 mul !cast_ua⁻¹ !cast_ua⁻¹
+  end
+
+  @[hott] def trivial_group_of_is_contr' (G : Group) [H : is_contr G] : G = G0 :=
+  eq_of_isomorphism (trivial_group_of_is_contr G)
+
+
+end group
