src/hott/types/int/hott.hlean
@@ -1,0 +1,178 @@
+/-
+Copyright (c) 2015 Floris van Doorn. All rights reserved.
+Released under Apache 2.0 license as described in the file LICENSE.
+Author: Floris van Doorn
+
+Theorems about the integers specific to HoTT
+-/
+#exit
+import .order types.eq arity algebra.bundled
+open core eq is_equiv equiv algebra is_trunc
+open nat (hiding pred)
+
+namespace int
+
+  section
+  open algebra
+  /-
+    we make these structures reducible, so that n * m in gℤ and agℤ can be interpreted as
+    multiplication on ℤ. For this it's needed that the carriers of gℤ and agℤ reduce to ℤ unfolding
+    only reducible definitions.
+  -/
+  @[hott] def group_integers [reducible] : AddGroup :=
+  AddGroup.mk ℤ _
+
+  notation `gℤ` := group_integers
+
+  @[hott] def AbGroup_int [reducible] : AddAbGroup :=
+  AddAbGroup.mk ℤ _
+
+  notation `agℤ` := AbGroup_int
+
+  @[hott] def ring_int : Ring :=
+  Ring.mk ℤ _
+
+  notation `rℤ` := ring_int
+
+  end
+
+  @[hott] def is_equiv_succ [instance] : is_equiv succ :=
+  adjointify succ pred (λa, !add_sub_cancel) (λa, !sub_add_cancel)
+  @[hott] def equiv_succ : ℤ ≃ ℤ := equiv.mk succ _
+
+  @[hott] def is_equiv_neg [instance] : is_equiv (neg : ℤ → ℤ) :=
+  adjointify neg neg (λx, !neg_neg) (λa, !neg_neg)
+  @[hott] def equiv_neg : ℤ ≃ ℤ := equiv.mk neg _
+
+  @[hott] def iiterate {A : Type _} (f : A ≃ A) (a : ℤ) : A ≃ A :=
+  rec_nat_on a erfl
+               (λb g, f ⬝e g)
+               (λb g, g ⬝e f⁻¹ᵉ)
+
+  @[hott] def max0 : ℤ → ℕ
+  | (of_nat n) := n
+  | (-[1+ n])  := 0
+
+  @[hott] lemma le_max0 : Π(n : ℤ), n ≤ of_nat (max0 n)
+  | (of_nat n) := proof le.refl n qed
+  | (-[1+ n])  := proof unit.star qed
+
+  @[hott] lemma le_of_max0_le {n : ℤ} {m : ℕ} (h : max0 n ≤ m) : n ≤ of_nat m :=
+  le.trans (le_max0 n) (of_nat_le_of_nat_of_le h)
+
+  -- @[hott] def iterate_trans {A : Type _} (f : A ≃ A) (a : ℤ)
+  --   : iterate f a ⬝e f = iterate f (a + 1) :=
+  -- sorry
+
+  -- @[hott] def trans_iterate {A : Type _} (f : A ≃ A) (a : ℤ)
+  --   : f ⬝e iterate f a = iterate f (a + 1) :=
+  -- sorry
+
+  -- @[hott] def iterate_trans_symm {A : Type _} (f : A ≃ A) (a : ℤ)
+  --   : iterate f a ⬝e f⁻¹e = iterate f (a - 1) :=
+  -- sorry
+
+  -- @[hott] def symm_trans_iterate {A : Type _} (f : A ≃ A) (a : ℤ)
+  --   : f⁻¹e ⬝e iterate f a = iterate f (a - 1) :=
+  -- sorry
+
+  -- @[hott] def iterate_neg {A : Type _} (f : A ≃ A) (a : ℤ)
+  --   : iterate f (-a) = (iterate f a)⁻¹e :=
+  -- rec_nat_on a idp
+  --   (λn p, calc
+  --     iterate f (-succ n) = iterate f (-n) ⬝e f⁻¹e : rec_nat_on_neg
+  --       ... = (iterate f n)⁻¹e ⬝e f⁻¹e : by rewrite p
+  --       ... = (f ⬝e iterate f n)⁻¹e : sorry
+  --       ... = (iterate f (succ n))⁻¹e : idp)
+  --   sorry
+
+  -- @[hott] def iterate_add {A : Type _} (f : A ≃ A) (a b : ℤ)
+  --   : iterate f (a + b) = equiv.trans (iterate f a) (iterate f b) :=
+  -- sorry
+
+  -- @[hott] def iterate_sub {A : Type _} (f : A ≃ A) (a b : ℤ)
+  --   : iterate f (a - b) = equiv.trans (iterate f a) (equiv.symm (iterate f b)) :=
+  -- sorry
+
+  -- @[hott] def iterate_mul {A : Type _} (f : A ≃ A) (a b : ℤ)
+  --   : iterate f (a * b) = iterate (iterate f a) b :=
+  -- sorry
+
+end int open int
+
+
+
+namespace eq
+  variables {A : Type _} {a : A} (p : a = a) (b c : ℤ) (n : ℕ)
+  @[hott] def power : a = a :=
+  rec_nat_on b idp
+               (λc q, q ⬝ p)
+               (λc q, q ⬝ p⁻¹)
+  --iterate (equiv_eq_closed_right p a) b idp
+
+  -- @[hott] def power_neg_succ (n : ℕ) : power p (-succ n) = power p (-n) ⬝ p⁻¹ :=
+  -- !rec_nat_on_neg
+
+  -- local attribute nat.add int.add int.of_num nat.of_num int.succ
+
+  @[hott] def power_con : power p b ⬝ p = power p (succ b) :=
+  rec_nat_on b
+    idp
+    (λn IH, idp)
+    (λn IH, calc
+      power p (-succ n) ⬝ p
+            = (power p (-int.of_nat n) ⬝ p⁻¹) ⬝ p : by krewrite [↑power,rec_nat_on_neg]
+        ... = power p (-int.of_nat n) : inv_con_cancel_right
+        ... = power p (succ (-succ n)) : by rewrite -succ_neg_succ)
+
+  @[hott] def power_con_inv : power p b ⬝ p⁻¹ = power p (pred b) :=
+  rec_nat_on b
+    idp
+    (λn IH, calc
+      power p (succ n) ⬝ p⁻¹ = power p n : by apply con_inv_cancel_right
+        ... = power p (pred (succ n))   : by rewrite pred_nat_succ)
+    (λn IH, calc
+      power p (-int.of_nat (succ n)) ⬝ p⁻¹
+            = power p (-int.of_nat (succ (succ n))) : by krewrite [↑power,*rec_nat_on_neg]
+        ... = power p (pred (-succ n)) : by rewrite -neg_succ)
+
+  @[hott] def con_power : p ⬝ power p b = power p (succ b) :=
+  rec_nat_on b
+  ( by rewrite ↑[power];exact !idp_con⁻¹)
+  ( λn IH, proof calc
+    p ⬝ power p (succ n) = (p ⬝ power p n) ⬝ p : con.assoc p _ p
+      ... = power p (succ (succ n)) : by rewrite IH qed)
+  ( λn IH, calc
+          p ⬝ power p (-int.of_nat (succ n))
+                = p ⬝ (power p (-int.of_nat n) ⬝ p⁻¹) : by rewrite [↑power, rec_nat_on_neg]
+            ... = (p ⬝ power p (-int.of_nat n)) ⬝ p⁻¹ : con.assoc
+            ... = power p (succ (-int.of_nat n)) ⬝ p⁻¹ : by rewrite IH
+            ... = power p (pred (succ (-int.of_nat n))) : power_con_inv
+            ... = power p (succ (-int.of_nat (succ n))) : by rewrite [succ_neg_nat_succ,int.pred_succ])
+
+  @[hott] def inv_con_power : p⁻¹ ⬝ power p b = power p (pred b) :=
+  rec_nat_on b
+  ( by rewrite ↑[power];exact !idp_con⁻¹)
+  (λn IH, calc
+    p⁻¹ ⬝ power p (succ n) = p⁻¹ ⬝ power p n ⬝ p : con.assoc
+      ... = power p (pred n) ⬝ p : by rewrite IH
+      ... = power p (succ (pred n)) : power_con
+      ... = power p (pred (succ n)) : by rewrite [succ_pred,-int.pred_succ n])
+  ( λn IH, calc
+    p⁻¹ ⬝ power p (-int.of_nat (succ n))
+          = p⁻¹ ⬝ (power p (-int.of_nat n) ⬝ p⁻¹) : by rewrite [↑power,rec_nat_on_neg]
+      ... = (p⁻¹ ⬝ power p (-int.of_nat n)) ⬝ p⁻¹ : con.assoc
+      ... = power p (pred (-int.of_nat n)) ⬝ p⁻¹ : by rewrite IH
+      ... = power p (-int.of_nat (succ n)) ⬝ p⁻¹ : by rewrite -neg_succ
+      ... = power p (-succ (succ n)) : by krewrite [↑power,*rec_nat_on_neg]
+      ... = power p (pred (-succ n)) : by rewrite -neg_succ)
+
+  @[hott] def power_con_power : Π(b : ℤ), power p b ⬝ power p c = power p (b + c) :=
+  rec_nat_on c
+    (λb, by rewrite int.add_zero)
+    (λn IH b, by rewrite [-con_power,-con.assoc,power_con,IH,↑succ,add.assoc,
+                          add.comm (int.of_nat n)])
+    (λn IH b, by rewrite [neg_nat_succ,-inv_con_power,-con.assoc,power_con_inv,IH,↑pred,
+                          +sub_eq_add_neg,add.assoc,add.comm (-n)])
+
+end eq
